Update interop stubs to handle taint

src/arch/x64/interop/Main.ml
@@ -16,82 +16,81 @@ let memcpy = ("memcpy", [("dst", TBuffer TUInt64, Sec); ("src", TBuffer TUInt64,
     Stk (Prims.parse_int "18"))
 *)
 
-let gctr_bytes_extra_buffer = ("gctr_bytes_extra_buffer_win", [
-  ("plain_b", TBuffer TUInt128); ("num_bytes", TBase TUInt64);
-  ("iv_old", TGhost "quad32"); ("iv_b", TBuffer TUInt128);
-  ("key", TGhost "aes_key_LE AES_128"); ("keys_b", TBuffer TUInt128);
-  ("cipher_b", TBuffer TUInt128)], Stk (Prims.parse_int "0"))
 
-(*
 let aes_encrypt_block = ("aes128_encrypt_block_win", [
-  ("output_b", TBuffer TUInt128); ("input_b", TBuffer TUInt128);
-  ("key", TGhost "aes_key_LE AES_128"); ("keys_b", TBuffer TUInt128)
+  ("output_b", TBuffer TUInt128, Sec); ("input_b", TBuffer TUInt128, Sec);
+  ("key", TGhost "aes_key_LE AES_128", Pub); ("keys_b", TBuffer TUInt128, Sec)
   ], Stk (Prims.parse_int "0"))
 
 
-
+(*
 let ghash = ("ghash_incremental_bytes_stdcall_win", [
-  ("h_b", TBuffer TUInt128); ("hash_b", TBuffer TUInt128);
-  ("input_b", TBuffer TUInt128); ("num_bytes", TBase TUInt64)
+  ("h_b", TBuffer TUInt128, Sec); ("hash_b", TBuffer TUInt128, Sec);
+  ("input_b", TBuffer TUInt128, Sec); ("num_bytes", TBase TUInt64, Pub)
   ], Stk (Prims.parse_int "5"))
 *)
+
 (*
-let gctr_bytes_extra_buffer = ("gctr_bytes_extra_buffer", [
-  ("plain_b", TBuffer TUInt128); ("num_bytes", TBase TUInt64);
-  ("iv_old", TGhost "quad32"); ("iv_b", TBuffer TUInt128);
-  ("key", TGhost "aes_key_LE AES_128"); ("keys_b", TBuffer TUInt128);
-  ("cipher_b", TBuffer TUInt128)], Stk (Prims.parse_int "0"))
+let gctr_bytes_extra_buffer = ("gctr_bytes_extra_buffer_win", [
+  ("plain_b", TBuffer TUInt128, Sec); ("num_bytes", TBase TUInt64, Pub);
+  ("iv_old", TGhost "quad32", Pub); ("iv_b", TBuffer TUInt128, Sec);
+  ("key", TGhost "aes_key_LE AES_128", Pub); ("keys_b", TBuffer TUInt128, Sec);
+  ("cipher_b", TBuffer TUInt128, Sec)], Stk (Prims.parse_int "0"))
 *)
+
 (*
 let ghash_extra = ("ghash_incremental_extra_stdcall_win", [
-  ("in_b", TBuffer TUInt128); ("hash_b", TBuffer TUInt128);
-  ("h_b", TBuffer TUInt128); ("num_bytes", TBase TUInt64);
-  ("orig_hash", TGhost "quad32")], Stk (Prims.parse_int "4"))
+  ("in_b", TBuffer TUInt128, Sec); ("hash_b", TBuffer TUInt128, Sec);
+  ("h_b", TBuffer TUInt128, Sec); ("num_bytes", TBase TUInt64, Pub);
+  ("orig_hash", TGhost "quad32", Pub)], Stk (Prims.parse_int "4"))
 *)
+
 (*
 let ghash_one_block = ("ghash_incremental_one_block_buffer_win", [
-  ("h_b", TBuffer TUInt128); ("hash_b", TBuffer TUInt128);
-  ("input_b", TBuffer TUInt128); ("offset", TBase TUInt64)
+  ("h_b", TBuffer TUInt128, Sec); ("hash_b", TBuffer TUInt128, Sec);
+  ("input_b", TBuffer TUInt128, Sec); ("offset", TBase TUInt64, Pub)
   ], Stk (Prims.parse_int "4"))
 *)
+
 (*
-let inc32 = ("inc32_buffer_win", [("iv_b", TBuffer TUInt128)], Stk (Prims.parse_int "0"))
+let inc32 = ("inc32_buffer_win", [("iv_b", TBuffer TUInt128, Sec)], Stk (Prims.parse_int "0"))
 *)
 
 (* 
-let quad32_xor = ("quad32_xor_buffer_win", [("src1", TBuffer TUInt128);
-  ("src2", TBuffer TUInt128); ("dst", TBuffer TUInt128)], Stk (Prims.parse_int "0"))
+let quad32_xor = ("quad32_xor_buffer_win", [("src1", TBuffer TUInt128, Sec);
+  ("src2", TBuffer TUInt128, Sec); ("dst", TBuffer TUInt128, Sec)], Stk (Prims.parse_int "0"))
 *)
 
 (*
 let gcm_make_length = ("gcm_make_length_quad_buffer_win", [
-  ("plain_num_bytes", TBase TUInt64); ("auth_num_bytes", TBase TUInt64);
-  ("b", TBuffer TUInt128)], Stk (Prims.parse_int "0"))
+  ("plain_num_bytes", TBase TUInt64, Pub); ("auth_num_bytes", TBase TUInt64, Pub);
+  ("b", TBuffer TUInt128, Sec)], Stk (Prims.parse_int "0"))
 *)
 
 (*
 let gcm_load_xor = ("gcm_load_xor_store_buffer_win", [
-  ("plain_b", TBuffer TUInt128); ("mask_b", TBuffer TUInt128);
-  ("cipher_b", TBuffer TUInt128); ("offset", TBase TUInt64);
-  ("num_blocks", TGhost "nat64");
-  ("key", TGhost "aes_key_LE AES_128"); ("iv", TGhost "quad32")], Stk (Prims.parse_int "0"))
+  ("plain_b", TBuffer TUInt128, Sec); ("mask_b", TBuffer TUInt128, Sec);
+  ("cipher_b", TBuffer TUInt128, Sec); ("offset", TBase TUInt64, Sec);
+  ("num_blocks", TGhost "nat64", Pub);
+  ("key", TGhost "aes_key_LE AES_128", Pub); ("iv", TGhost "quad32", Pub)], Stk (Prims.parse_int "0"))
 *)
 
 (*
-
 let aes_encrypt_block_be = ("aes128_encrypt_block_be_win", [
-  ("output_b", TBuffer TUInt128); ("input_b", TBuffer TUInt128);
-  ("key", TGhost "aes_key_LE AES_128"); ("keys_b", TBuffer TUInt128)
+  ("output_b", TBuffer TUInt128, Sec); ("input_b", TBuffer TUInt128, Sec);
+  ("key", TGhost "aes_key_LE AES_128", Pub); ("keys_b", TBuffer TUInt128, Sec)
   ], Stk (Prims.parse_int "0"))
 *)
+
 (*
-let mk_quad1 = ("mk_quad32_lo0_be_1_buffer_win", [("b", TBuffer TUInt128)], Stk (Prims.parse_int "0")) *)
+let mk_quad1 = ("mk_quad32_lo0_be_1_buffer_win", [("b", TBuffer TUInt128, Sec)], Stk (Prims.parse_int "0"))
+*)
 (*
-let zero_quad32_buffer = ("zero_quad32_buffer_win", [("b", TBuffer TUInt128)], Stk (Prims.parse_int "0"))
+let zero_quad32_buffer = ("zero_quad32_buffer_win", [("b", TBuffer TUInt128, Sec)], Stk (Prims.parse_int "0"))
 *)
 let os = Windows 
 
-let name = gctr_bytes_extra_buffer 
+let name = aes_encrypt_block 
 
 let _ = print_string (translate_vale os X86 name)
 let _ = print_newline()
