src/arch/x64/interop/AESEncryptBlock_win.fst
@@ -8,6 +8,7 @@ module M = LowStar.Modifies
 open LowStar.ModifiesPat
 open FStar.HyperStack.ST
 module HS = FStar.HyperStack
+module S8 = SecretByte
 open Interop
 open Words_s
 open Types_s
@@ -20,9 +21,7 @@ open BufferViewHelpers
 
 open Vale_aes128_encrypt_block_win
 
-assume val st_put (h:HS.mem) (p:HS.mem -> Type0) (f:(h0:HS.mem{p h0}) -> GTot HS.mem) : Stack unit (fun h0 -> p h0 /\ h == h0) (fun h0 _ h1 -> h == h0 /\ f h == h1)
-
-let b8 = B.buffer UInt8.t
+assume val st_put (p:HS.mem -> Type0) (f:(h0:HS.mem{p h0}) -> GTot HS.mem) : Stack unit (fun h0 -> p h0) (fun h0 _ h1 -> f h0 == h1)
 
 //The map from buffers to addresses in the heap, that remains abstract
 assume val addrs: addr_map
@@ -33,47 +32,14 @@ assume val init_xmms:xmm -> quad32
 
 #set-options "--initial_fuel 6 --max_fuel 6 --initial_ifuel 2 --max_ifuel 2"
 // TODO: Prove these two lemmas if they are not proven automatically
-let implies_pre (h0:HS.mem) (output_b:b8) (input_b:b8) (key:Ghost.erased (aes_key_LE AES_128)) (keys_b:b8)  (stack_b:b8) : Lemma
+let implies_pre (h0:HS.mem) (output_b:s8) (input_b:s8) (key:Ghost.erased (aes_key_LE AES_128)) (keys_b:s8)  (stack_b:b8) : Lemma
   (requires pre_cond h0 output_b input_b key keys_b /\ B.length stack_b == 32 /\ live h0 stack_b /\ buf_disjoint_from stack_b [output_b;input_b;keys_b])
   (ensures (
-B.length stack_b == 32 /\ live h0 stack_b /\ buf_disjoint_from stack_b [output_b;input_b;keys_b] /\ (  let buffers = stack_b::output_b::input_b::keys_b::[] in
-  let (mem:mem) = {addrs = addrs; ptrs = buffers; hs = h0} in
-  let addr_output_b = addrs output_b in
-  let addr_input_b = addrs input_b in
-  let addr_keys_b = addrs keys_b in
-  let addr_stack:nat64 = addrs stack_b + 0 in
-  let regs = fun r -> begin match r with
-    | Rsp -> addr_stack
-    | Rcx -> addr_output_b
-    | Rdx -> addr_input_b
-    | R8 -> addr_keys_b
-    | _ -> init_regs r end in
-  let xmms = init_xmms in
-  let s0 = {ok = true; regs = regs; xmms = xmms; flags = 0; mem = mem} in
-  length_t_eq (TBase TUInt64) stack_b;
-  length_t_eq (TBase TUInt128) output_b;
-  length_t_eq (TBase TUInt128) input_b;
-  length_t_eq (TBase TUInt128) keys_b;
-  va_pre (va_code_aes128_encrypt_block_win ()) s0 stack_b output_b input_b (Ghost.reveal key) keys_b ))) =
-  length_t_eq (TBase TUInt64) stack_b;
-  length_t_eq (TBase TUInt128) output_b;
-  length_t_eq (TBase TUInt128) input_b;
-  length_t_eq (TBase TUInt128) keys_b;
-  ()
-
-let implies_post (va_s0:va_state) (va_sM:va_state) (va_fM:va_fuel) (output_b:b8) (input_b:b8) (key:Ghost.erased (aes_key_LE AES_128)) (keys_b:b8)  (stack_b:b8) : Lemma
-  (requires pre_cond va_s0.mem.hs output_b input_b key keys_b /\ B.length stack_b == 32 /\ live va_s0.mem.hs stack_b /\ buf_disjoint_from stack_b [output_b;input_b;keys_b]/\
-    va_post (va_code_aes128_encrypt_block_win ()) va_s0 va_sM va_fM stack_b output_b input_b (Ghost.reveal key) keys_b )
-  (ensures post_cond va_s0.mem.hs va_sM.mem.hs output_b input_b key keys_b ) =
-  length_t_eq (TBase TUInt64) stack_b;
-  length_t_eq (TBase TUInt128) output_b;
-  length_t_eq (TBase TUInt128) input_b;
-  length_t_eq (TBase TUInt128) keys_b;
-  ()
-
-val ghost_aes128_encrypt_block_win: output_b:b8 -> input_b:b8 -> key:Ghost.erased (aes_key_LE AES_128) -> keys_b:b8 ->  stack_b:b8 -> (h0:HS.mem{pre_cond h0 output_b input_b key keys_b /\ B.length stack_b == 32 /\ live h0 stack_b /\ buf_disjoint_from stack_b [output_b;input_b;keys_b]}) -> GTot (h1:HS.mem{post_cond h0 h1 output_b input_b key keys_b })
-
-let ghost_aes128_encrypt_block_win output_b input_b key keys_b stack_b h0 =
+B.length stack_b == 32 /\ live h0 stack_b /\ buf_disjoint_from stack_b [output_b;input_b;keys_b] /\ (  let taint_func (x:b8) : GTot taint =
+    if StrongExcludedMiddle.strong_excluded_middle (x == output_b) then Secret else
+    if StrongExcludedMiddle.strong_excluded_middle (x == input_b) then Secret else
+    if StrongExcludedMiddle.strong_excluded_middle (x == keys_b) then Secret else
+    Public in
   let buffers = stack_b::output_b::input_b::keys_b::[] in
   let (mem:mem) = {addrs = addrs; ptrs = buffers; hs = h0} in
   let addr_output_b = addrs output_b in
@@ -87,7 +53,50 @@ let ghost_aes128_encrypt_block_win output_b input_b key keys_b stack_b h0 =
     | R8 -> addr_keys_b
     | _ -> init_regs r end in
   let xmms = init_xmms in
-  let s0 = {ok = true; regs = regs; xmms = xmms; flags = 0; mem = mem} in
+  let s0 = {ok = true; regs = regs; xmms = xmms; flags = 0; mem = mem; trace = []; memTaint = create_valid_memtaint mem buffers taint_func} in
+  length_t_eq (TBase TUInt64) stack_b;
+  length_t_eq (TBase TUInt128) output_b;
+  length_t_eq (TBase TUInt128) input_b;
+  length_t_eq (TBase TUInt128) keys_b;
+  va_pre (va_code_aes128_encrypt_block_win ()) s0 stack_b output_b input_b (Ghost.reveal key) keys_b ))) =
+  length_t_eq (TBase TUInt64) stack_b;
+  length_t_eq (TBase TUInt128) output_b;
+  length_t_eq (TBase TUInt128) input_b;
+  length_t_eq (TBase TUInt128) keys_b;
+  ()
+
+let implies_post (va_s0:va_state) (va_sM:va_state) (va_fM:va_fuel) (output_b:s8) (input_b:s8) (key:Ghost.erased (aes_key_LE AES_128)) (keys_b:s8)  (stack_b:b8) : Lemma
+  (requires pre_cond va_s0.mem.hs output_b input_b key keys_b /\ B.length stack_b == 32 /\ live va_s0.mem.hs stack_b /\ buf_disjoint_from stack_b [output_b;input_b;keys_b]/\
+    va_post (va_code_aes128_encrypt_block_win ()) va_s0 va_sM va_fM stack_b output_b input_b (Ghost.reveal key) keys_b )
+  (ensures post_cond va_s0.mem.hs va_sM.mem.hs output_b input_b key keys_b ) =
+  length_t_eq (TBase TUInt64) stack_b;
+  length_t_eq (TBase TUInt128) output_b;
+  length_t_eq (TBase TUInt128) input_b;
+  length_t_eq (TBase TUInt128) keys_b;
+  ()
+
+val ghost_aes128_encrypt_block_win: output_b:s8 -> input_b:s8 -> key:Ghost.erased (aes_key_LE AES_128) -> keys_b:s8 ->  stack_b:b8 -> (h0:HS.mem{pre_cond h0 output_b input_b key keys_b /\ B.length stack_b == 32 /\ live h0 stack_b /\ buf_disjoint_from stack_b [output_b;input_b;keys_b]}) -> GTot (h1:HS.mem{post_cond h0 h1 output_b input_b key keys_b })
+
+let ghost_aes128_encrypt_block_win output_b input_b key keys_b stack_b h0 =
+  let taint_func (x:b8) : GTot taint =
+    if StrongExcludedMiddle.strong_excluded_middle (x == output_b) then Secret else
+    if StrongExcludedMiddle.strong_excluded_middle (x == input_b) then Secret else
+    if StrongExcludedMiddle.strong_excluded_middle (x == keys_b) then Secret else
+    Public in
+  let buffers = stack_b::output_b::input_b::keys_b::[] in
+  let (mem:mem) = {addrs = addrs; ptrs = buffers; hs = h0} in
+  let addr_output_b = addrs output_b in
+  let addr_input_b = addrs input_b in
+  let addr_keys_b = addrs keys_b in
+  let addr_stack:nat64 = addrs stack_b + 0 in
+  let regs = fun r -> begin match r with
+    | Rsp -> addr_stack
+    | Rcx -> addr_output_b
+    | Rdx -> addr_input_b
+    | R8 -> addr_keys_b
+    | _ -> init_regs r end in
+  let xmms = init_xmms in
+  let s0 = {ok = true; regs = regs; xmms = xmms; flags = 0; mem = mem; trace = []; memTaint = create_valid_memtaint mem buffers taint_func} in
   length_t_eq (TBase TUInt64) stack_b;
   length_t_eq (TBase TUInt128) output_b;
   length_t_eq (TBase TUInt128) input_b;
@@ -125,5 +134,5 @@ let aes128_encrypt_block_win output_b input_b key keys_b  =
   push_frame();
   let (stack_b:b8) = B.alloca (UInt8.uint_to_t 0) (UInt32.uint_to_t 32) in
   let h0 = get() in
-  st_put h0 (fun h -> pre_cond h output_b input_b key keys_b /\ B.length stack_b == 32 /\ live h stack_b /\ buf_disjoint_from stack_b [output_b;input_b;keys_b]) (ghost_aes128_encrypt_block_win output_b input_b key keys_b stack_b);
+  st_put (fun h -> pre_cond h output_b input_b key keys_b /\ B.length stack_b == 32 /\ live h stack_b /\ buf_disjoint_from stack_b [output_b;input_b;keys_b]) (ghost_aes128_encrypt_block_win output_b input_b key keys_b stack_b);
   pop_frame()
