src/arch/x64/interop/GCTR_win.fst
@@ -8,6 +8,7 @@ module M = LowStar.Modifies
 open LowStar.ModifiesPat
 open FStar.HyperStack.ST
 module HS = FStar.HyperStack
+module S8 = SecretByte
 open Interop
 open Words_s
 open Types_s
@@ -20,9 +21,7 @@ open BufferViewHelpers
 
 open Vale_gctr_bytes_extra_buffer_win
 
-assume val st_put (h:HS.mem) (p:HS.mem -> Type0) (f:(h0:HS.mem{p h0}) -> GTot HS.mem) : Stack unit (fun h0 -> p h0 /\ h == h0) (fun h0 _ h1 -> h == h0 /\ f h == h1)
-
-let b8 = B.buffer UInt8.t
+assume val st_put (p:HS.mem -> Type0) (f:(h0:HS.mem{p h0}) -> GTot HS.mem) : Stack unit (fun h0 -> p h0) (fun h0 _ h1 -> f h0 == h1)
 
 //The map from buffers to addresses in the heap, that remains abstract
 assume val addrs: addr_map
@@ -32,33 +31,15 @@ assume val init_regs:reg -> nat64
 assume val init_xmms:xmm -> quad32
 
 #set-options "--initial_fuel 7 --max_fuel 7 --initial_ifuel 2 --max_ifuel 2"
-// TODO: Prove these two lemmas if they are not proven automatically
-let implies_pre (h0:HS.mem) (plain_b:b8) (num_bytes:nat64) (iv_old:Ghost.erased (quad32)) (iv_b:b8) (key:Ghost.erased (aes_key_LE AES_128)) (keys_b:b8) (cipher_b:b8)  (stack_b:b8) : Lemma
+let implies_pre (h0:HS.mem) (plain_b:s8) (num_bytes:nat64) (iv_old:Ghost.erased (quad32)) (iv_b:s8) (key:Ghost.erased (aes_key_LE AES_128)) (keys_b:s8) (cipher_b:s8)  (stack_b:b8) : Lemma
   (requires pre_cond h0 plain_b num_bytes iv_old iv_b key keys_b cipher_b /\ B.length stack_b == 48 /\ live h0 stack_b /\ buf_disjoint_from stack_b [plain_b;iv_b;keys_b;cipher_b])
   (ensures (
-B.length stack_b == 48 /\ live h0 stack_b /\ buf_disjoint_from stack_b [plain_b;iv_b;keys_b;cipher_b] /\ (  let buffers = stack_b::plain_b::iv_b::keys_b::cipher_b::[] in
-  let (mem:mem) = {addrs = addrs; ptrs = buffers; hs = h0} in
-  let addr_plain_b = addrs plain_b in
-  let addr_iv_b = addrs iv_b in
-  let addr_keys_b = addrs keys_b in
-  let addr_cipher_b = addrs cipher_b in
-  let addr_stack:nat64 = addrs stack_b + 0 in
-  let regs = fun r -> begin match r with
-    | Rsp -> addr_stack
-    | Rcx -> addr_plain_b
-    | Rdx -> num_bytes
-    | R8 -> addr_iv_b
-    | R9 -> addr_keys_b
-    | _ -> init_regs r end in
-  let mem = buffer_write #(TBase TUInt64) stack_b 5 (addrs cipher_b) mem in
-  let xmms = init_xmms in
-  let s0 = {ok = true; regs = regs; xmms = xmms; flags = 0; mem = mem} in
-  length_t_eq (TBase TUInt64) stack_b;
-  length_t_eq (TBase TUInt128) plain_b;
-  length_t_eq (TBase TUInt128) iv_b;
-  length_t_eq (TBase TUInt128) keys_b;
-  length_t_eq (TBase TUInt128) cipher_b;
-  va_pre (va_code_gctr_bytes_extra_buffer_win ()) s0 stack_b plain_b num_bytes (Ghost.reveal iv_old) iv_b (Ghost.reveal key) keys_b cipher_b ))) =
+B.length stack_b == 48 /\ live h0 stack_b /\ buf_disjoint_from stack_b [plain_b;iv_b;keys_b;cipher_b] /\ (  let taint_func (x:b8) : GTot taint =
+    if StrongExcludedMiddle.strong_excluded_middle (x == plain_b) then Secret else
+    if StrongExcludedMiddle.strong_excluded_middle (x == iv_b) then Secret else
+    if StrongExcludedMiddle.strong_excluded_middle (x == keys_b) then Secret else
+    if StrongExcludedMiddle.strong_excluded_middle (x == cipher_b) then Secret else
+    Public in
   let buffers = stack_b::plain_b::iv_b::keys_b::cipher_b::[] in
   let (mem:mem) = {addrs = addrs; ptrs = buffers; hs = h0} in
   let addr_plain_b = addrs plain_b in
@@ -75,7 +56,40 @@ B.length stack_b == 48 /\ live h0 stack_b /\ buf_disjoint_from stack_b [plain_b;
     | _ -> init_regs r end in
   let mem = buffer_write #(TBase TUInt64) stack_b 5 (addrs cipher_b) mem in
   let xmms = init_xmms in
-  let va_s0 = {ok = true; regs = regs; xmms = xmms; flags = 0; mem = mem} in  
+  let s0 = {ok = true; regs = regs; xmms = xmms; flags = 0; mem = mem; trace = []; memTaint = create_valid_memtaint mem buffers taint_func} in
+  length_t_eq (TBase TUInt64) stack_b;
+  length_t_eq (TBase TUInt128) plain_b;
+  length_t_eq (TBase TUInt128) iv_b;
+  length_t_eq (TBase TUInt128) keys_b;
+  length_t_eq (TBase TUInt128) cipher_b;
+  va_pre (va_code_gctr_bytes_extra_buffer_win ()) s0 stack_b plain_b num_bytes (Ghost.reveal iv_old) iv_b (Ghost.reveal key) keys_b cipher_b ))) =
+  let taint_func (x:b8) : GTot taint =
+    if StrongExcludedMiddle.strong_excluded_middle (x == plain_b) then Secret else
+    if StrongExcludedMiddle.strong_excluded_middle (x == iv_b) then Secret else
+    if StrongExcludedMiddle.strong_excluded_middle (x == keys_b) then Secret else
+    if StrongExcludedMiddle.strong_excluded_middle (x == cipher_b) then Secret else
+    Public in
+  let buffers = stack_b::plain_b::iv_b::keys_b::cipher_b::[] in
+  let (mem:mem) = {addrs = addrs; ptrs = buffers; hs = h0} in
+  let addr_plain_b = addrs plain_b in
+  let addr_iv_b = addrs iv_b in
+  let addr_keys_b = addrs keys_b in
+  let addr_cipher_b = addrs cipher_b in
+  let addr_stack:nat64 = addrs stack_b + 0 in
+  let regs = fun r -> begin match r with
+    | Rsp -> addr_stack
+    | Rcx -> addr_plain_b
+    | Rdx -> num_bytes
+    | R8 -> addr_iv_b
+    | R9 -> addr_keys_b
+    | _ -> init_regs r end in
+  let mem = buffer_write #(TBase TUInt64) stack_b 5 (addrs cipher_b) mem in
+  let xmms = init_xmms in
+  let va_s0 = {ok = true; regs = regs; xmms = xmms; flags = 0; mem = mem; trace = []; memTaint = create_valid_memtaint mem buffers taint_func} in
+  assert (B.disjoint stack_b plain_b);
+  assert (B.disjoint stack_b iv_b);
+  assert (B.disjoint stack_b keys_b);
+  assert (B.disjoint stack_b cipher_b);
   length_t_eq (TBase TUInt64) stack_b;
   length_t_eq (TBase TUInt128) plain_b;
   length_t_eq (TBase TUInt128) iv_b;
@@ -88,12 +102,18 @@ B.length stack_b == 48 /\ live h0 stack_b /\ buf_disjoint_from stack_b [plain_b;
   assert (Seq.equal (buffer_as_seq (va_get_mem va_s0) iv_b) (BV.as_seq h0 iv128_b));
   BV.as_seq_sel h0 iv128_b 0;
   let keys128_b = BV.mk_buffer_view keys_b Views.view128 in
-  assert (Seq.equal (buffer_as_seq (va_get_mem va_s0) keys_b) (BV.as_seq h0 keys128_b));  
+  assert (Seq.equal (buffer_as_seq (va_get_mem va_s0) keys_b) (BV.as_seq h0 keys128_b));    
   ()
 
-let implies_post (h0:HS.mem) (va_sM:va_state) (va_fM:va_fuel) (plain_b:b8) (num_bytes:nat64) (iv_old:Ghost.erased (quad32)) (iv_b:b8) (key:Ghost.erased (aes_key_LE AES_128)) (keys_b:b8) (cipher_b:b8)  (stack_b:b8) : Lemma
+let implies_post (h0:HS.mem) (va_sM:va_state) (va_fM:va_fuel) (plain_b:s8) (num_bytes:nat64) (iv_old:Ghost.erased (quad32)) (iv_b:s8) (key:Ghost.erased (aes_key_LE AES_128)) (keys_b:s8) (cipher_b:s8)  (stack_b:b8) : Lemma
   (requires pre_cond h0 plain_b num_bytes iv_old iv_b key keys_b cipher_b /\ B.length stack_b == 48 /\ live h0 stack_b /\ buf_disjoint_from stack_b [plain_b;iv_b;keys_b;cipher_b]/\
-(
+(  let taint_func (x:b8) : GTot taint =
+    if StrongExcludedMiddle.strong_excluded_middle (x == plain_b) then Secret else
+    if StrongExcludedMiddle.strong_excluded_middle (x == iv_b) then Secret else
+    if StrongExcludedMiddle.strong_excluded_middle (x == keys_b) then Secret else
+    if StrongExcludedMiddle.strong_excluded_middle (x == cipher_b) then Secret else
+    if StrongExcludedMiddle.strong_excluded_middle (x == stack_b) then Public else
+    Public in
   let buffers = stack_b::plain_b::iv_b::keys_b::cipher_b::[] in
   let (mem:mem) = {addrs = addrs; ptrs = buffers; hs = h0} in
   let addr_plain_b = addrs plain_b in
@@ -110,14 +130,16 @@ let implies_post (h0:HS.mem) (va_sM:va_state) (va_fM:va_fuel) (plain_b:b8) (num_
     | _ -> init_regs r end in
   let mem = buffer_write #(TBase TUInt64) stack_b 5 (addrs cipher_b) mem in
   let xmms = init_xmms in
-  let s0 = {ok = true; regs = regs; xmms = xmms; flags = 0; mem = mem} in
-  length_t_eq (TBase TUInt64) stack_b;
-  length_t_eq (TBase TUInt128) plain_b;
-  length_t_eq (TBase TUInt128) iv_b;
-  length_t_eq (TBase TUInt128) keys_b;
-  length_t_eq (TBase TUInt128) cipher_b;
-    va_post (va_code_gctr_bytes_extra_buffer_win ()) s0 va_sM va_fM stack_b plain_b num_bytes (Ghost.reveal iv_old) iv_b (Ghost.reveal key) keys_b cipher_b ))
+  let va_s0 = {ok = true; regs = regs; xmms = xmms; flags = 0; mem = mem; trace = []; memTaint = create_valid_memtaint mem buffers taint_func} in    
+    va_post (va_code_gctr_bytes_extra_buffer_win ()) va_s0 va_sM va_fM stack_b plain_b num_bytes (Ghost.reveal iv_old) iv_b (Ghost.reveal key) keys_b cipher_b) )
   (ensures post_cond h0 va_sM.mem.hs plain_b num_bytes iv_old iv_b key keys_b cipher_b ) =
+  let taint_func (x:b8) : GTot taint =
+    if StrongExcludedMiddle.strong_excluded_middle (x == plain_b) then Secret else
+    if StrongExcludedMiddle.strong_excluded_middle (x == iv_b) then Secret else
+    if StrongExcludedMiddle.strong_excluded_middle (x == keys_b) then Secret else
+    if StrongExcludedMiddle.strong_excluded_middle (x == cipher_b) then Secret else
+    if StrongExcludedMiddle.strong_excluded_middle (x == stack_b) then Public else
+    Public in
   let buffers = stack_b::plain_b::iv_b::keys_b::cipher_b::[] in
   let (mem:mem) = {addrs = addrs; ptrs = buffers; hs = h0} in
   let addr_plain_b = addrs plain_b in
@@ -134,7 +156,7 @@ let implies_post (h0:HS.mem) (va_sM:va_state) (va_fM:va_fuel) (plain_b:b8) (num_
     | _ -> init_regs r end in
   let mem = buffer_write #(TBase TUInt64) stack_b 5 (addrs cipher_b) mem in
   let xmms = init_xmms in
-  let va_s0 = {ok = true; regs = regs; xmms = xmms; flags = 0; mem = mem} in   
+  let va_s0 = {ok = true; regs = regs; xmms = xmms; flags = 0; mem = mem; trace = []; memTaint = create_valid_memtaint mem buffers taint_func} in  
   length_t_eq (TBase TUInt64) stack_b;
   length_t_eq (TBase TUInt128) plain_b;
   length_t_eq (TBase TUInt128) iv_b;
@@ -142,12 +164,19 @@ let implies_post (h0:HS.mem) (va_sM:va_state) (va_fM:va_fuel) (plain_b:b8) (num_
   length_t_eq (TBase TUInt128) cipher_b;
   assert (Seq.equal (buffer_to_seq_quad32 cipher_b h0) (buffer128_as_seq (va_get_mem va_s0) cipher_b));
   assert (Seq.equal (buffer_to_seq_quad32 cipher_b va_sM.mem.hs) (buffer128_as_seq (va_get_mem va_sM) cipher_b));
-  assert (Seq.equal (buffer_to_seq_quad32 plain_b h0) (buffer128_as_seq (va_get_mem va_s0) plain_b));    
+  assert (Seq.equal (buffer_to_seq_quad32 plain_b h0) (buffer128_as_seq (va_get_mem va_s0) plain_b));  
   ()
 
-val ghost_gctr_bytes_extra_buffer_win: plain_b:b8 -> num_bytes:nat64 -> iv_old:Ghost.erased (quad32) -> iv_b:b8 -> key:Ghost.erased (aes_key_LE AES_128) -> keys_b:b8 -> cipher_b:b8 ->  stack_b:b8 -> (h0:HS.mem{pre_cond h0 plain_b num_bytes iv_old iv_b key keys_b cipher_b /\ B.length stack_b == 48 /\ live h0 stack_b /\ buf_disjoint_from stack_b [plain_b;iv_b;keys_b;cipher_b]}) -> GTot (h1:HS.mem{post_cond h0 h1 plain_b num_bytes iv_old iv_b key keys_b cipher_b  /\ M.modifies (M.loc_union (M.loc_buffer cipher_b) (M.loc_buffer stack_b)) h0 h1 })
+val ghost_gctr_bytes_extra_buffer_win: plain_b:s8 -> num_bytes:nat64 -> iv_old:Ghost.erased (quad32) -> iv_b:s8 -> key:Ghost.erased (aes_key_LE AES_128) -> keys_b:s8 -> cipher_b:s8 ->  stack_b:b8 -> (h0:HS.mem{pre_cond h0 plain_b num_bytes iv_old iv_b key keys_b cipher_b /\ B.length stack_b == 48 /\ live h0 stack_b /\ buf_disjoint_from stack_b [plain_b;iv_b;keys_b;cipher_b]}) -> GTot (h1:HS.mem{post_cond h0 h1 plain_b num_bytes iv_old iv_b key keys_b cipher_b  /\ M.modifies (M.loc_union (M.loc_buffer cipher_b) (M.loc_buffer stack_b)) h0 h1})
 
 let ghost_gctr_bytes_extra_buffer_win plain_b num_bytes iv_old iv_b key keys_b cipher_b stack_b h0 =
+  let taint_func (x:b8) : GTot taint =
+    if StrongExcludedMiddle.strong_excluded_middle (x == plain_b) then Secret else
+    if StrongExcludedMiddle.strong_excluded_middle (x == iv_b) then Secret else
+    if StrongExcludedMiddle.strong_excluded_middle (x == keys_b) then Secret else
+    if StrongExcludedMiddle.strong_excluded_middle (x == cipher_b) then Secret else
+    if StrongExcludedMiddle.strong_excluded_middle (x == stack_b) then Public else
+    Public in
   let buffers = stack_b::plain_b::iv_b::keys_b::cipher_b::[] in
   let (mem:mem) = {addrs = addrs; ptrs = buffers; hs = h0} in
   let addr_plain_b = addrs plain_b in
@@ -164,7 +193,7 @@ let ghost_gctr_bytes_extra_buffer_win plain_b num_bytes iv_old iv_b key keys_b c
     | _ -> init_regs r end in
   let mem = buffer_write #(TBase TUInt64) stack_b 5 (addrs cipher_b) mem in
   let xmms = init_xmms in
-  let s0 = {ok = true; regs = regs; xmms = xmms; flags = 0; mem = mem} in
+  let s0 = {ok = true; regs = regs; xmms = xmms; flags = 0; mem = mem; trace = []; memTaint = create_valid_memtaint mem buffers taint_func} in
   length_t_eq (TBase TUInt64) stack_b;
   length_t_eq (TBase TUInt128) plain_b;
   length_t_eq (TBase TUInt128) iv_b;
@@ -203,5 +232,5 @@ let gctr_bytes_extra_buffer_win plain_b num_bytes iv_old iv_b key keys_b cipher_
   push_frame();
   let (stack_b:b8) = B.alloca (UInt8.uint_to_t 0) (UInt32.uint_to_t 48) in
   let h0 = get() in
-  st_put h0 (fun h -> pre_cond h plain_b (UInt64.v num_bytes) iv_old iv_b key keys_b cipher_b /\ B.length stack_b == 48 /\ live h stack_b /\ buf_disjoint_from stack_b [plain_b;iv_b;keys_b;cipher_b]) (ghost_gctr_bytes_extra_buffer_win plain_b (UInt64.v num_bytes) iv_old iv_b key keys_b cipher_b stack_b);
+  st_put (fun h -> pre_cond h plain_b (UInt64.v num_bytes) iv_old iv_b key keys_b cipher_b /\ B.length stack_b == 48 /\ live h stack_b /\ buf_disjoint_from stack_b [plain_b;iv_b;keys_b;cipher_b]) (ghost_gctr_bytes_extra_buffer_win plain_b (UInt64.v num_bytes) iv_old iv_b key keys_b cipher_b stack_b);
   pop_frame()
