src/arch/x64/interop/GHash_extra_win.fst
@@ -8,6 +8,7 @@ module M = LowStar.Modifies
 open LowStar.ModifiesPat
 open FStar.HyperStack.ST
 module HS = FStar.HyperStack
+module S8 = SecretByte
 open Interop
 open Words_s
 open Types_s
@@ -20,9 +21,7 @@ open BufferViewHelpers
 
 open Vale_ghash_incremental_extra_stdcall_win
 
-assume val st_put (h:HS.mem) (p:HS.mem -> Type0) (f:(h0:HS.mem{p h0}) -> GTot HS.mem) : Stack unit (fun h0 -> p h0 /\ h == h0) (fun h0 _ h1 -> h == h0 /\ f h == h1)
-
-let b8 = B.buffer UInt8.t
+assume val st_put (p:HS.mem -> Type0) (f:(h0:HS.mem{p h0}) -> GTot HS.mem) : Stack unit (fun h0 -> p h0) (fun h0 _ h1 -> f h0 == h1)
 
 //The map from buffers to addresses in the heap, that remains abstract
 assume val addrs: addr_map
@@ -33,29 +32,14 @@ assume val init_xmms:xmm -> quad32
 
 #set-options "--initial_fuel 6 --max_fuel 6 --initial_ifuel 2 --max_ifuel 2"
 // TODO: Prove these two lemmas if they are not proven automatically
-let implies_pre (h0:HS.mem) (in_b:b8) (hash_b:b8) (h_b:b8) (num_bytes:nat64) (orig_hash:Ghost.erased (quad32))  (stack_b:b8) : Lemma
+let implies_pre (h0:HS.mem) (in_b:s8) (hash_b:s8) (h_b:s8) (num_bytes:nat64) (orig_hash:Ghost.erased (quad32))  (stack_b:b8) : Lemma
   (requires pre_cond h0 in_b hash_b h_b num_bytes orig_hash /\ B.length stack_b == 72 /\ live h0 stack_b /\ buf_disjoint_from stack_b [in_b;hash_b;h_b])
   (ensures (
-B.length stack_b == 72 /\ live h0 stack_b /\ buf_disjoint_from stack_b [in_b;hash_b;h_b] /\ (  let buffers = stack_b::in_b::hash_b::h_b::[] in
-  let (mem:mem) = {addrs = addrs; ptrs = buffers; hs = h0} in
-  let addr_in_b = addrs in_b in
-  let addr_hash_b = addrs hash_b in
-  let addr_h_b = addrs h_b in
-  let addr_stack:nat64 = addrs stack_b + 32 in
-  let regs = fun r -> begin match r with
-    | Rsp -> addr_stack
-    | Rcx -> addr_in_b
-    | Rdx -> addr_hash_b
-    | R8 -> addr_h_b
-    | R9 -> num_bytes
-    | _ -> init_regs r end in
-  let xmms = init_xmms in
-  let s0 = {ok = true; regs = regs; xmms = xmms; flags = 0; mem = mem} in
-  length_t_eq (TBase TUInt64) stack_b;
-  length_t_eq (TBase TUInt128) in_b;
-  length_t_eq (TBase TUInt128) hash_b;
-  length_t_eq (TBase TUInt128) h_b;
-  va_pre (va_code_ghash_incremental_extra_stdcall_win ()) s0 stack_b in_b hash_b h_b num_bytes (Ghost.reveal orig_hash) ))) =
+B.length stack_b == 72 /\ live h0 stack_b /\ buf_disjoint_from stack_b [in_b;hash_b;h_b] /\ (  let taint_func (x:b8) : GTot taint =
+    if StrongExcludedMiddle.strong_excluded_middle (x == in_b) then Secret else
+    if StrongExcludedMiddle.strong_excluded_middle (x == hash_b) then Secret else
+    if StrongExcludedMiddle.strong_excluded_middle (x == h_b) then Secret else
+    Public in
   let buffers = stack_b::in_b::hash_b::h_b::[] in
   let (mem:mem) = {addrs = addrs; ptrs = buffers; hs = h0} in
   let addr_in_b = addrs in_b in
@@ -70,7 +54,32 @@ B.length stack_b == 72 /\ live h0 stack_b /\ buf_disjoint_from stack_b [in_b;has
     | R9 -> num_bytes
     | _ -> init_regs r end in
   let xmms = init_xmms in
-  let s0 = {ok = true; regs = regs; xmms = xmms; flags = 0; mem = mem} in  
+  let s0 = {ok = true; regs = regs; xmms = xmms; flags = 0; mem = mem; trace = []; memTaint = create_valid_memtaint mem buffers taint_func} in
+  length_t_eq (TBase TUInt64) stack_b;
+  length_t_eq (TBase TUInt128) in_b;
+  length_t_eq (TBase TUInt128) hash_b;
+  length_t_eq (TBase TUInt128) h_b;
+  va_pre (va_code_ghash_incremental_extra_stdcall_win ()) s0 stack_b in_b hash_b h_b num_bytes (Ghost.reveal orig_hash) ))) =
+  let taint_func (x:b8) : GTot taint =
+    if StrongExcludedMiddle.strong_excluded_middle (x == in_b) then Secret else
+    if StrongExcludedMiddle.strong_excluded_middle (x == hash_b) then Secret else
+    if StrongExcludedMiddle.strong_excluded_middle (x == h_b) then Secret else
+    Public in
+  let buffers = stack_b::in_b::hash_b::h_b::[] in
+  let (mem:mem) = {addrs = addrs; ptrs = buffers; hs = h0} in
+  let addr_in_b = addrs in_b in
+  let addr_hash_b = addrs hash_b in
+  let addr_h_b = addrs h_b in
+  let addr_stack:nat64 = addrs stack_b + 32 in
+  let regs = fun r -> begin match r with
+    | Rsp -> addr_stack
+    | Rcx -> addr_in_b
+    | Rdx -> addr_hash_b
+    | R8 -> addr_h_b
+    | R9 -> num_bytes
+    | _ -> init_regs r end in
+  let xmms = init_xmms in
+  let s0 = {ok = true; regs = regs; xmms = xmms; flags = 0; mem = mem; trace = []; memTaint = create_valid_memtaint mem buffers taint_func} in  
   length_t_eq (TBase TUInt64) stack_b;
   length_t_eq (TBase TUInt128) in_b;
   length_t_eq (TBase TUInt128) hash_b;
@@ -81,10 +90,10 @@ B.length stack_b == 72 /\ live h0 stack_b /\ buf_disjoint_from stack_b [in_b;has
   BV.as_seq_sel h0 h128_b 0;  
   let hash128_b = BV.mk_buffer_view hash_b Views.view128 in
   assert (Seq.equal (buffer_as_seq (va_get_mem s0) hash_b) (BV.as_seq h0 hash128_b));
-  BV.as_seq_sel h0 hash128_b 0;    
+  BV.as_seq_sel h0 hash128_b 0;   
   ()
 
-let implies_post (va_s0:va_state) (va_sM:va_state) (va_fM:va_fuel) (in_b:b8) (hash_b:b8) (h_b:b8) (num_bytes:nat64) (orig_hash:Ghost.erased (quad32))  (stack_b:b8) : Lemma
+let implies_post (va_s0:va_state) (va_sM:va_state) (va_fM:va_fuel) (in_b:s8) (hash_b:s8) (h_b:s8) (num_bytes:nat64) (orig_hash:Ghost.erased (quad32))  (stack_b:b8) : Lemma
   (requires pre_cond va_s0.mem.hs in_b hash_b h_b num_bytes orig_hash /\ B.length stack_b == 72 /\ live va_s0.mem.hs stack_b /\ buf_disjoint_from stack_b [in_b;hash_b;h_b]/\
     va_post (va_code_ghash_incremental_extra_stdcall_win ()) va_s0 va_sM va_fM stack_b in_b hash_b h_b num_bytes (Ghost.reveal orig_hash) )
   (ensures post_cond va_s0.mem.hs va_sM.mem.hs in_b hash_b h_b num_bytes orig_hash ) =
@@ -100,12 +109,17 @@ let implies_post (va_s0:va_state) (va_sM:va_state) (va_fM:va_fuel) (in_b:b8) (ha
   BV.as_seq_sel va_sM.mem.hs hash128_b 0;
   let h128_b = BV.mk_buffer_view h_b Views.view128 in
   assert (Seq.equal (buffer_as_seq (va_get_mem va_s0) h_b) (BV.as_seq va_s0.mem.hs h128_b));
-  BV.as_seq_sel va_s0.mem.hs h128_b 0;  
+  BV.as_seq_sel va_s0.mem.hs h128_b 0;   
   ()
 
-val ghost_ghash_incremental_extra_stdcall_win: in_b:b8 -> hash_b:b8 -> h_b:b8 -> num_bytes:nat64 -> orig_hash:Ghost.erased (quad32) ->  stack_b:b8 -> (h0:HS.mem{pre_cond h0 in_b hash_b h_b num_bytes orig_hash /\ B.length stack_b == 72 /\ live h0 stack_b /\ buf_disjoint_from stack_b [in_b;hash_b;h_b]}) -> GTot (h1:HS.mem{post_cond h0 h1 in_b hash_b h_b num_bytes orig_hash /\ M.modifies (M.loc_union (M.loc_buffer hash_b) (M.loc_buffer stack_b)) h0 h1})
+val ghost_ghash_incremental_extra_stdcall_win: in_b:s8 -> hash_b:s8 -> h_b:s8 -> num_bytes:nat64 -> orig_hash:Ghost.erased (quad32) ->  stack_b:b8 -> (h0:HS.mem{pre_cond h0 in_b hash_b h_b num_bytes orig_hash /\ B.length stack_b == 72 /\ live h0 stack_b /\ buf_disjoint_from stack_b [in_b;hash_b;h_b]}) -> GTot (h1:HS.mem{post_cond h0 h1 in_b hash_b h_b num_bytes orig_hash /\ M.modifies (M.loc_union (M.loc_buffer hash_b) (M.loc_buffer stack_b)) h0 h1 })
 
 let ghost_ghash_incremental_extra_stdcall_win in_b hash_b h_b num_bytes orig_hash stack_b h0 =
+  let taint_func (x:b8) : GTot taint =
+    if StrongExcludedMiddle.strong_excluded_middle (x == in_b) then Secret else
+    if StrongExcludedMiddle.strong_excluded_middle (x == hash_b) then Secret else
+    if StrongExcludedMiddle.strong_excluded_middle (x == h_b) then Secret else
+    Public in
   let buffers = stack_b::in_b::hash_b::h_b::[] in
   let (mem:mem) = {addrs = addrs; ptrs = buffers; hs = h0} in
   let addr_in_b = addrs in_b in
@@ -120,7 +134,7 @@ let ghost_ghash_incremental_extra_stdcall_win in_b hash_b h_b num_bytes orig_has
     | R9 -> num_bytes
     | _ -> init_regs r end in
   let xmms = init_xmms in
-  let s0 = {ok = true; regs = regs; xmms = xmms; flags = 0; mem = mem} in
+  let s0 = {ok = true; regs = regs; xmms = xmms; flags = 0; mem = mem; trace = []; memTaint = create_valid_memtaint mem buffers taint_func} in
   length_t_eq (TBase TUInt64) stack_b;
   length_t_eq (TBase TUInt128) in_b;
   length_t_eq (TBase TUInt128) hash_b;
@@ -158,5 +172,5 @@ let ghash_incremental_extra_stdcall_win in_b hash_b h_b num_bytes orig_hash  =
   push_frame();
   let (stack_b:b8) = B.alloca (UInt8.uint_to_t 0) (UInt32.uint_to_t 72) in
   let h0 = get() in
-  st_put h0 (fun h -> pre_cond h in_b hash_b h_b (UInt64.v num_bytes) orig_hash /\ B.length stack_b == 72 /\ live h stack_b /\ buf_disjoint_from stack_b [in_b;hash_b;h_b]) (ghost_ghash_incremental_extra_stdcall_win in_b hash_b h_b (UInt64.v num_bytes) orig_hash stack_b);
+  st_put (fun h -> pre_cond h in_b hash_b h_b (UInt64.v num_bytes) orig_hash /\ B.length stack_b == 72 /\ live h stack_b /\ buf_disjoint_from stack_b [in_b;hash_b;h_b]) (ghost_ghash_incremental_extra_stdcall_win in_b hash_b h_b (UInt64.v num_bytes) orig_hash stack_b);
   pop_frame()
