src/arch/x64/interop/GHash_extra_win.fsti
@@ -8,6 +8,7 @@ module M = LowStar.Modifies
 open LowStar.ModifiesPat
 open FStar.HyperStack.ST
 module HS = FStar.HyperStack
+module S8 = SecretByte
 open Interop
 open Words_s
 open Words.Seq_s
@@ -23,24 +24,25 @@ open GCM_s
 open GCM_helpers_i
 open GHash_i
 
+let s8 = B.buffer S8.t
 
-let rec loc_locs_disjoint_rec (l:b8) (ls:list b8) : Type0 =
+let rec loc_locs_disjoint_rec (l:s8) (ls:list s8) : Type0 =
   match ls with
   | [] -> True
   | h::t -> M.loc_disjoint (M.loc_buffer l) (M.loc_buffer h) /\ loc_locs_disjoint_rec l t
 
-let rec locs_disjoint_rec (ls:list b8) : Type0 =
+let rec locs_disjoint_rec (ls:list s8) : Type0 =
   match ls with
   | [] -> True
   | h::t -> loc_locs_disjoint_rec h t /\ locs_disjoint_rec t
 
 unfold
-let bufs_disjoint (ls:list b8) : Type0 = normalize (locs_disjoint_rec ls)
+let bufs_disjoint (ls:list s8) : Type0 = normalize (locs_disjoint_rec ls)
 
 unfold
-let buf_disjoint_from (b:b8) (ls:list b8) : Type0 = normalize (loc_locs_disjoint_rec b ls)
+let buf_disjoint_from (b:s8) (ls:list s8) : Type0 = normalize (loc_locs_disjoint_rec b ls)
 
-let buffer_to_quad32 (b:B.buffer UInt8.t { B.length b % 16 == 0 /\ B.length b > 0 }) (h:HS.mem) : GTot quad32 =
+let buffer_to_quad32 (b:s8 { B.length b % 16 == 0 /\ B.length b > 0 }) (h:HS.mem) : GTot quad32 =
   let b128 = BV.mk_buffer_view b Views.view128 in
   BV.as_buffer_mk_buffer_view b Views.view128;
   BV.get_view_mk_buffer_view b Views.view128;
@@ -49,7 +51,7 @@ let buffer_to_quad32 (b:B.buffer UInt8.t { B.length b % 16 == 0 /\ B.length b > 
   assert (BV.length b128 > 0);
   BV.sel h b128 0
 
-let buffer_to_seq_quad32 (b:B.buffer UInt8.t { B.length b % 16 == 0 }) (h:HS.mem) : GTot (s:Seq.seq quad32 {Seq.length s == B.length b / 16} ) =
+let buffer_to_seq_quad32 (b:s8 { B.length b % 16 == 0 }) (h:HS.mem) : GTot (s:Seq.seq quad32 {Seq.length s == B.length b / 16} ) =
   let b128 = BV.mk_buffer_view b Views.view128 in
   BV.as_buffer_mk_buffer_view b Views.view128;
   BV.get_view_mk_buffer_view b Views.view128;
@@ -59,7 +61,7 @@ let buffer_to_seq_quad32 (b:B.buffer UInt8.t { B.length b % 16 == 0 }) (h:HS.mem
 open FStar.Mul
 
 // TODO: Complete with your pre- and post-conditions
-let pre_cond (h:HS.mem) (in_b:b8) (hash_b:b8) (h_b:b8) (num_bytes:nat64) (orig_hash:Ghost.erased (quad32)) = live h in_b /\ live h hash_b /\ live h h_b /\ bufs_disjoint [in_b;hash_b;h_b] /\ length in_b % 16 == 0 /\ length hash_b % 16 == 0 /\ length h_b % 16 == 0 /\
+let pre_cond (h:HS.mem) (in_b:s8) (hash_b:s8) (h_b:s8) (num_bytes:nat64) (orig_hash:Ghost.erased (quad32)) = live h in_b /\ live h hash_b /\ live h h_b /\ bufs_disjoint [in_b;hash_b;h_b] /\ length in_b % 16 == 0 /\ length hash_b % 16 == 0 /\ length h_b % 16 == 0 /\
    ( let mods = M.loc_buffer hash_b in 
     B.live h in_b /\ B.live h hash_b /\ B.live h h_b /\ 
     M.loc_disjoint (M.loc_buffer in_b) mods /\
@@ -92,7 +94,7 @@ let pre_cond (h:HS.mem) (in_b:b8) (hash_b:b8) (h_b:b8) (num_bytes:nat64) (orig_h
     )
 )
 
-let post_cond (h:HS.mem) (h':HS.mem) (in_b:b8) (hash_b:b8) (h_b:b8) (num_bytes:nat64) (orig_hash:Ghost.erased (quad32)) = length in_b % 16 == 0 /\ length hash_b % 16 == 0 /\ length h_b % 16 == 0 /\
+let post_cond (h:HS.mem) (h':HS.mem) (in_b:s8) (hash_b:s8) (h_b:s8) (num_bytes:nat64) (orig_hash:Ghost.erased (quad32)) = length in_b % 16 == 0 /\ length hash_b % 16 == 0 /\ length h_b % 16 == 0 /\
     B.length in_b  == bytes_to_quad_size num_bytes * 16 /\
     B.length h_b == 16 /\
     B.length hash_b == 16 /\
@@ -111,10 +113,10 @@ let post_cond (h:HS.mem) (h':HS.mem) (in_b:b8) (hash_b:b8) (h_b:b8) (num_bytes:n
     )
   ) 
 
-let full_post_cond (h:HS.mem) (h':HS.mem) (in_b:b8) (hash_b:b8) (h_b:b8) (num_bytes:nat64) (orig_hash:Ghost.erased (quad32)) = 
+let full_post_cond (h:HS.mem) (h':HS.mem) (in_b:s8) (hash_b:s8) (h_b:s8) (num_bytes:nat64) (orig_hash:Ghost.erased (quad32)) = 
     let mods = M.loc_buffer hash_b in
     M.modifies mods h h' /\ post_cond h h' in_b hash_b h_b num_bytes orig_hash
 
-val ghash_incremental_extra_stdcall_win: in_b:b8 -> hash_b:b8 -> h_b:b8 -> num_bytes:UInt64.t -> orig_hash:Ghost.erased (quad32) -> Stack unit
+val ghash_incremental_extra_stdcall_win: in_b:s8 -> hash_b:s8 -> h_b:s8 -> num_bytes:UInt64.t -> orig_hash:Ghost.erased (quad32) -> Stack unit
 	(requires (fun h -> pre_cond h in_b hash_b h_b (UInt64.v num_bytes) orig_hash ))
 	(ensures (fun h0 _ h1 -> full_post_cond h0 h1 in_b hash_b h_b (UInt64.v num_bytes) orig_hash ))
