src/arch/x64/interop/GHash_one_block_win.fsti
@@ -8,6 +8,7 @@ module M = LowStar.Modifies
 open LowStar.ModifiesPat
 open FStar.HyperStack.ST
 module HS = FStar.HyperStack
+module S8 = SecretByte
 open Interop
 open Words_s
 open Types_s
@@ -17,28 +18,28 @@ open X64.Vale.State_i
 open X64.Vale.Decls_i
 open GHash_i
 
+let s8 = B.buffer S8.t
 
-
-let rec loc_locs_disjoint_rec (l:b8) (ls:list b8) : Type0 =
+let rec loc_locs_disjoint_rec (l:s8) (ls:list s8) : Type0 =
   match ls with
   | [] -> True
   | h::t -> M.loc_disjoint (M.loc_buffer l) (M.loc_buffer h) /\ loc_locs_disjoint_rec l t
 
-let rec locs_disjoint_rec (ls:list b8) : Type0 =
+let rec locs_disjoint_rec (ls:list s8) : Type0 =
   match ls with
   | [] -> True
   | h::t -> loc_locs_disjoint_rec h t /\ locs_disjoint_rec t
 
 unfold
-let bufs_disjoint (ls:list b8) : Type0 = normalize (locs_disjoint_rec ls)
+let bufs_disjoint (ls:list s8) : Type0 = normalize (locs_disjoint_rec ls)
 
 unfold
-let buf_disjoint_from (b:b8) (ls:list b8) : Type0 = normalize (loc_locs_disjoint_rec b ls)
+let buf_disjoint_from (b:s8) (ls:list s8) : Type0 = normalize (loc_locs_disjoint_rec b ls)
 
 open FStar.Mul
 
 
-let buffer_to_quad32 (b:B.buffer UInt8.t { B.length b % 16 == 0 /\ B.length b > 0 }) (h:HS.mem) : GTot quad32 =
+let buffer_to_quad32 (b:s8{ B.length b % 16 == 0 /\ B.length b > 0 }) (h:HS.mem) : GTot quad32 =
   let b128 = BV.mk_buffer_view b Views.view128 in
   BV.as_buffer_mk_buffer_view b Views.view128;
   BV.get_view_mk_buffer_view b Views.view128;
@@ -48,17 +49,17 @@ let buffer_to_quad32 (b:B.buffer UInt8.t { B.length b % 16 == 0 /\ B.length b > 
   BV.sel h b128 0
   //index (BV.as_seq h b128) 0
 
-let buffer_to_seq_quad32 (b:B.buffer UInt8.t { B.length b % 16 == 0 }) (h:HS.mem) : GTot (s:Seq.seq quad32 {Seq.length s == B.length b / 16} ) =
+let buffer_to_seq_quad32 (b:s8{ B.length b % 16 == 0 }) (h:HS.mem) : GTot (s:Seq.seq quad32 {Seq.length s == B.length b / 16} ) =
   let b128 = BV.mk_buffer_view b Views.view128 in
   BV.as_buffer_mk_buffer_view b Views.view128;
   BV.get_view_mk_buffer_view b Views.view128;
   BV.length_eq b128;
   (BV.as_seq h b128)
 
-let pre_cond (h:HS.mem) (h_b:b8) (hash_b:b8) (input_b:b8) (offset:nat64) = live h h_b /\ live h hash_b /\ live h input_b /\ bufs_disjoint [h_b;hash_b;input_b] /\ length h_b % 16 == 0 /\ length hash_b % 16 == 0 /\ length input_b % 16 == 0 /\
+let pre_cond (h:HS.mem) (h_b:s8) (hash_b:s8) (input_b:s8) (offset:nat64) = live h h_b /\ live h hash_b /\ live h input_b /\ bufs_disjoint [h_b;hash_b;input_b] /\ length h_b % 16 == 0 /\ length hash_b % 16 == 0 /\ length input_b % 16 == 0 /\
   B.length h_b >= 16 /\ B.length hash_b >= 16 /\ B.length input_b >= 16 * (offset + 1)
 
-let partial_post_cond (h:HS.mem) (h':HS.mem) (h_b:b8) (hash_b:b8) (input_b:b8) (offset:nat64) = length h_b % 16 == 0 /\ length hash_b % 16 == 0 /\ length input_b % 16 == 0 /\
+let partial_post_cond (h:HS.mem) (h':HS.mem) (h_b:s8) (hash_b:s8) (input_b:s8) (offset:nat64) = length h_b % 16 == 0 /\ length hash_b % 16 == 0 /\ length input_b % 16 == 0 /\
  B.length h_b >= 16 /\ B.length hash_b >= 16 /\ B.length input_b >= 16 * (offset + 1) /\
     (let old_hash = buffer_to_quad32 hash_b h  in
      let new_hash = buffer_to_quad32 hash_b h' in
@@ -69,11 +70,11 @@ let partial_post_cond (h:HS.mem) (h':HS.mem) (h_b:b8) (hash_b:b8) (input_b:b8) (
     )
 
 
-let post_cond (h:HS.mem) (h':HS.mem) (h_b:b8) (hash_b:b8) (input_b:b8) (offset:nat64) =
+let post_cond (h:HS.mem) (h':HS.mem) (h_b:s8) (hash_b:s8) (input_b:s8) (offset:nat64) =
     M.modifies (M.loc_buffer hash_b) h h' /\
     partial_post_cond h h' h_b hash_b input_b offset
 
 
-val ghash_incremental_one_block_buffer_win: h_b:b8 -> hash_b:b8 -> input_b:b8 -> offset:UInt64.t -> Stack unit
+val ghash_incremental_one_block_buffer_win: h_b:s8 -> hash_b:s8 -> input_b:s8 -> offset:UInt64.t -> Stack unit
 	(requires (fun h -> pre_cond h h_b hash_b input_b (UInt64.v offset) ))
 	(ensures (fun h0 _ h1 -> post_cond h0 h1 h_b hash_b input_b (UInt64.v offset) ))
