src/arch/x64/interop/GHash_stdcall_win.fst
@@ -8,6 +8,7 @@ module M = LowStar.Modifies
 open LowStar.ModifiesPat
 open FStar.HyperStack.ST
 module HS = FStar.HyperStack
+module S8 = SecretByte
 open Interop
 open Words_s
 open Types_s
@@ -20,9 +21,7 @@ open BufferViewHelpers
 
 open Vale_ghash_incremental_bytes_stdcall_win
 
-assume val st_put (h:HS.mem) (p:HS.mem -> Type0) (f:(h0:HS.mem{p h0}) -> GTot HS.mem) : Stack unit (fun h0 -> p h0 /\ h == h0) (fun h0 _ h1 -> h == h0 /\ f h == h1)
-
-let b8 = B.buffer UInt8.t
+assume val st_put (p:HS.mem -> Type0) (f:(h0:HS.mem{p h0}) -> GTot HS.mem) : Stack unit (fun h0 -> p h0) (fun h0 _ h1 -> f h0 == h1)
 
 //The map from buffers to addresses in the heap, that remains abstract
 assume val addrs: addr_map
@@ -33,51 +32,14 @@ assume val init_xmms:xmm -> quad32
 
 #set-options "--initial_fuel 6 --max_fuel 6 --initial_ifuel 2 --max_ifuel 2"
 // TODO: Prove these two lemmas if they are not proven automatically
-let implies_pre (h0:HS.mem) (h_b:b8) (hash_b:b8) (input_b:b8) (num_bytes:nat64)  (stack_b:b8) : Lemma
+let implies_pre (h0:HS.mem) (h_b:s8) (hash_b:s8) (input_b:s8) (num_bytes:nat64)  (stack_b:b8) : Lemma
   (requires pre_cond h0 h_b hash_b input_b num_bytes /\ B.length stack_b == 80 /\ live h0 stack_b /\ buf_disjoint_from stack_b [h_b;hash_b;input_b])
   (ensures (
-B.length stack_b == 80 /\ live h0 stack_b /\ buf_disjoint_from stack_b [h_b;hash_b;input_b] /\ (  let buffers = stack_b::h_b::hash_b::input_b::[] in
-  let (mem:mem) = {addrs = addrs; ptrs = buffers; hs = h0} in
-  let addr_h_b = addrs h_b in
-  let addr_hash_b = addrs hash_b in
-  let addr_input_b = addrs input_b in
-  let addr_stack:nat64 = addrs stack_b + 40 in
-  let regs = fun r -> begin match r with
-    | Rsp -> addr_stack
-    | Rcx -> addr_h_b
-    | Rdx -> addr_hash_b
-    | R8 -> addr_input_b
-    | R9 -> num_bytes
-    | _ -> init_regs r end in
-  let xmms = init_xmms in
-  let s0 = {ok = true; regs = regs; xmms = xmms; flags = 0; mem = mem} in
-  length_t_eq (TBase TUInt64) stack_b;
-  length_t_eq (TBase TUInt128) h_b;
-  length_t_eq (TBase TUInt128) hash_b;
-  length_t_eq (TBase TUInt128) input_b;
-  va_pre (va_code_ghash_incremental_bytes_stdcall_win ()) s0 stack_b h_b hash_b input_b num_bytes ))) =
-  length_t_eq (TBase TUInt64) stack_b;
-  length_t_eq (TBase TUInt128) h_b;
-  length_t_eq (TBase TUInt128) hash_b;
-  length_t_eq (TBase TUInt128) input_b;
-  ()
-
-let implies_post (va_s0:va_state) (va_sM:va_state) (va_fM:va_fuel) (h_b:b8) (hash_b:b8) (input_b:b8) (num_bytes:nat64)  (stack_b:b8) : Lemma
-  (requires pre_cond va_s0.mem.hs h_b hash_b input_b num_bytes /\ B.length stack_b == 80 /\ live va_s0.mem.hs stack_b /\ buf_disjoint_from stack_b [h_b;hash_b;input_b]/\
-    va_post (va_code_ghash_incremental_bytes_stdcall_win ()) va_s0 va_sM va_fM stack_b h_b hash_b input_b num_bytes )
-  (ensures post_cond va_s0.mem.hs va_sM.mem.hs h_b hash_b input_b num_bytes ) =
-  length_t_eq (TBase TUInt64) stack_b;
-  length_t_eq (TBase TUInt128) h_b;
-  length_t_eq (TBase TUInt128) hash_b;
-  length_t_eq (TBase TUInt128) input_b;
-  assert (Seq.equal
-    (buffer128_as_seq (va_get_mem va_sM) input_b)
-    (buffer_to_seq_quad input_b va_s0.mem.hs));  
-  ()
-
-val ghost_ghash_incremental_bytes_stdcall_win: h_b:b8 -> hash_b:b8 -> input_b:b8 -> num_bytes:nat64 ->  stack_b:b8 -> (h0:HS.mem{pre_cond h0 h_b hash_b input_b num_bytes /\ B.length stack_b == 80 /\ live h0 stack_b /\ buf_disjoint_from stack_b [h_b;hash_b;input_b]}) -> GTot (h1:HS.mem{post_cond h0 h1 h_b hash_b input_b num_bytes /\ M.modifies (M.loc_union (M.loc_buffer hash_b) (M.loc_buffer stack_b)) h0 h1 })
-
-let ghost_ghash_incremental_bytes_stdcall_win h_b hash_b input_b num_bytes stack_b h0 =
+B.length stack_b == 80 /\ live h0 stack_b /\ buf_disjoint_from stack_b [h_b;hash_b;input_b] /\ (  let taint_func (x:b8) : GTot taint =
+    if StrongExcludedMiddle.strong_excluded_middle (x == h_b) then Secret else
+    if StrongExcludedMiddle.strong_excluded_middle (x == hash_b) then Secret else
+    if StrongExcludedMiddle.strong_excluded_middle (x == input_b) then Secret else
+    Public in
   let buffers = stack_b::h_b::hash_b::input_b::[] in
   let (mem:mem) = {addrs = addrs; ptrs = buffers; hs = h0} in
   let addr_h_b = addrs h_b in
@@ -92,7 +54,54 @@ let ghost_ghash_incremental_bytes_stdcall_win h_b hash_b input_b num_bytes stack
     | R9 -> num_bytes
     | _ -> init_regs r end in
   let xmms = init_xmms in
-  let s0 = {ok = true; regs = regs; xmms = xmms; flags = 0; mem = mem} in
+  let s0 = {ok = true; regs = regs; xmms = xmms; flags = 0; mem = mem; trace = []; memTaint = create_valid_memtaint mem buffers taint_func} in
+  length_t_eq (TBase TUInt64) stack_b;
+  length_t_eq (TBase TUInt128) h_b;
+  length_t_eq (TBase TUInt128) hash_b;
+  length_t_eq (TBase TUInt128) input_b;
+  va_pre (va_code_ghash_incremental_bytes_stdcall_win ()) s0 stack_b h_b hash_b input_b num_bytes ))) =
+  length_t_eq (TBase TUInt64) stack_b;
+  length_t_eq (TBase TUInt128) h_b;
+  length_t_eq (TBase TUInt128) hash_b;
+  length_t_eq (TBase TUInt128) input_b;
+  ()
+
+let implies_post (va_s0:va_state) (va_sM:va_state) (va_fM:va_fuel) (h_b:s8) (hash_b:s8) (input_b:s8) (num_bytes:nat64)  (stack_b:b8) : Lemma
+  (requires pre_cond va_s0.mem.hs h_b hash_b input_b num_bytes /\ B.length stack_b == 80 /\ live va_s0.mem.hs stack_b /\ buf_disjoint_from stack_b [h_b;hash_b;input_b]/\
+    va_post (va_code_ghash_incremental_bytes_stdcall_win ()) va_s0 va_sM va_fM stack_b h_b hash_b input_b num_bytes )
+  (ensures post_cond va_s0.mem.hs va_sM.mem.hs h_b hash_b input_b num_bytes ) =
+  length_t_eq (TBase TUInt64) stack_b;
+  length_t_eq (TBase TUInt128) h_b;
+  length_t_eq (TBase TUInt128) hash_b;
+  length_t_eq (TBase TUInt128) input_b;
+  assert (Seq.equal
+    (buffer128_as_seq (va_get_mem va_sM) input_b)
+    (buffer_to_seq_quad input_b va_s0.mem.hs));    
+  ()
+
+val ghost_ghash_incremental_bytes_stdcall_win: h_b:s8 -> hash_b:s8 -> input_b:s8 -> num_bytes:nat64 ->  stack_b:b8 -> (h0:HS.mem{pre_cond h0 h_b hash_b input_b num_bytes /\ B.length stack_b == 80 /\ live h0 stack_b /\ buf_disjoint_from stack_b [h_b;hash_b;input_b]}) -> GTot (h1:HS.mem{post_cond h0 h1 h_b hash_b input_b num_bytes  /\ M.modifies (M.loc_union (M.loc_buffer hash_b) (M.loc_buffer stack_b)) h0 h1})
+
+let ghost_ghash_incremental_bytes_stdcall_win h_b hash_b input_b num_bytes stack_b h0 =
+  let taint_func (x:b8) : GTot taint =
+    if StrongExcludedMiddle.strong_excluded_middle (x == h_b) then Secret else
+    if StrongExcludedMiddle.strong_excluded_middle (x == hash_b) then Secret else
+    if StrongExcludedMiddle.strong_excluded_middle (x == input_b) then Secret else
+    Public in
+  let buffers = stack_b::h_b::hash_b::input_b::[] in
+  let (mem:mem) = {addrs = addrs; ptrs = buffers; hs = h0} in
+  let addr_h_b = addrs h_b in
+  let addr_hash_b = addrs hash_b in
+  let addr_input_b = addrs input_b in
+  let addr_stack:nat64 = addrs stack_b + 40 in
+  let regs = fun r -> begin match r with
+    | Rsp -> addr_stack
+    | Rcx -> addr_h_b
+    | Rdx -> addr_hash_b
+    | R8 -> addr_input_b
+    | R9 -> num_bytes
+    | _ -> init_regs r end in
+  let xmms = init_xmms in
+  let s0 = {ok = true; regs = regs; xmms = xmms; flags = 0; mem = mem; trace = []; memTaint = create_valid_memtaint mem buffers taint_func} in
   length_t_eq (TBase TUInt64) stack_b;
   length_t_eq (TBase TUInt128) h_b;
   length_t_eq (TBase TUInt128) hash_b;
@@ -130,5 +139,5 @@ let ghash_incremental_bytes_stdcall_win h_b hash_b input_b num_bytes  =
   push_frame();
   let (stack_b:b8) = B.alloca (UInt8.uint_to_t 0) (UInt32.uint_to_t 80) in
   let h0 = get() in
-  st_put h0 (fun h -> pre_cond h h_b hash_b input_b (UInt64.v num_bytes) /\ B.length stack_b == 80 /\ live h stack_b /\ buf_disjoint_from stack_b [h_b;hash_b;input_b]) (ghost_ghash_incremental_bytes_stdcall_win h_b hash_b input_b (UInt64.v num_bytes) stack_b);
+  st_put (fun h -> pre_cond h h_b hash_b input_b (UInt64.v num_bytes) /\ B.length stack_b == 80 /\ live h stack_b /\ buf_disjoint_from stack_b [h_b;hash_b;input_b]) (ghost_ghash_incremental_bytes_stdcall_win h_b hash_b input_b (UInt64.v num_bytes) stack_b);
   pop_frame()
