src/arch/x64/interop/Gcm_load_xor_win.fst
@@ -8,13 +8,14 @@ module M = LowStar.Modifies
 open LowStar.ModifiesPat
 open FStar.HyperStack.ST
 module HS = FStar.HyperStack
+module S8 = SecretByte
 open Interop
 open Words_s
 open Types_s
 open X64.Machine_s
 open X64.Memory_i_s
 open X64.Vale.State_i
-//open X64.Vale.Decls_i
+open X64.Vale.Decls_i
 open BufferViewHelpers
 #set-options "--z3rlimit 40"
 
@@ -31,29 +32,14 @@ assume val init_xmms:xmm -> quad32
 
 #set-options "--initial_fuel 6 --max_fuel 6 --initial_ifuel 2 --max_ifuel 2"
 // TODO: Prove these two lemmas if they are not proven automatically
-let implies_pre (h0:HS.mem) (plain_b:b8) (mask_b:b8) (cipher_b:b8) (offset:nat64) (num_blocks:Ghost.erased (nat64)) (key:Ghost.erased (aes_key_LE AES_128)) (iv:Ghost.erased (quad32))  (stack_b:b8) : Lemma
-  (requires pre_cond h0 plain_b mask_b cipher_b offset num_blocks key iv /\ B.length stack_b == 40 /\ live h0 stack_b /\ bufs_disjoint [stack_b;plain_b;mask_b;cipher_b])
+let implies_pre (h0:HS.mem) (plain_b:s8) (mask_b:s8) (cipher_b:s8) (offset:nat64) (num_blocks:Ghost.erased (nat64)) (key:Ghost.erased (aes_key_LE AES_128)) (iv:Ghost.erased (quad32))  (stack_b:b8) : Lemma
+  (requires pre_cond h0 plain_b mask_b cipher_b offset num_blocks key iv /\ B.length stack_b == 40 /\ live h0 stack_b /\ buf_disjoint_from stack_b [plain_b;mask_b;cipher_b])
   (ensures (
-B.length stack_b == 40 /\ live h0 stack_b /\ bufs_disjoint [stack_b;plain_b;mask_b;cipher_b] /\ (  let buffers = stack_b::plain_b::mask_b::cipher_b::[] in
-  let (mem:mem) = {addrs = addrs; ptrs = buffers; hs = h0} in
-  let addr_plain_b = addrs plain_b in
-  let addr_mask_b = addrs mask_b in
-  let addr_cipher_b = addrs cipher_b in
-  let addr_stack:nat64 = addrs stack_b + 0 in
-  let regs = fun r -> begin match r with
-    | Rsp -> addr_stack
-    | Rcx -> addr_plain_b
-    | Rdx -> addr_mask_b
-    | R8 -> addr_cipher_b
-    | R9 -> offset
-    | _ -> init_regs r end in
-  let xmms = init_xmms in
-  let s0 = {ok = true; regs = regs; xmms = xmms; flags = 0; mem = mem} in
-  length_t_eq (TBase TUInt64) stack_b;
-  length_t_eq (TBase TUInt128) plain_b;
-  length_t_eq (TBase TUInt128) mask_b;
-  length_t_eq (TBase TUInt128) cipher_b;
-  va_pre (va_code_gcm_load_xor_store_buffer_win ()) s0 stack_b plain_b mask_b cipher_b offset (Ghost.reveal num_blocks) (Ghost.reveal key) (Ghost.reveal iv) ))) =
+B.length stack_b == 40 /\ live h0 stack_b /\ buf_disjoint_from stack_b [plain_b;mask_b;cipher_b] /\ (  let taint_func (x:b8) : GTot taint =
+    if StrongExcludedMiddle.strong_excluded_middle (x == plain_b) then Secret else
+    if StrongExcludedMiddle.strong_excluded_middle (x == mask_b) then Secret else
+    if StrongExcludedMiddle.strong_excluded_middle (x == cipher_b) then Secret else
+    Public in
   let buffers = stack_b::plain_b::mask_b::cipher_b::[] in
   let (mem:mem) = {addrs = addrs; ptrs = buffers; hs = h0} in
   let addr_plain_b = addrs plain_b in
@@ -68,7 +54,32 @@ B.length stack_b == 40 /\ live h0 stack_b /\ bufs_disjoint [stack_b;plain_b;mask
     | R9 -> offset
     | _ -> init_regs r end in
   let xmms = init_xmms in
-  let va_s0 = {ok = true; regs = regs; xmms = xmms; flags = 0; mem = mem} in  
+  let s0 = {ok = true; regs = regs; xmms = xmms; flags = 0; mem = mem; trace = []; memTaint = create_valid_memtaint mem buffers taint_func} in
+  length_t_eq (TBase TUInt64) stack_b;
+  length_t_eq (TBase TUInt128) plain_b;
+  length_t_eq (TBase TUInt128) mask_b;
+  length_t_eq (TBase TUInt128) cipher_b;
+  va_pre (va_code_gcm_load_xor_store_buffer_win ()) s0 stack_b plain_b mask_b cipher_b offset (Ghost.reveal num_blocks) (Ghost.reveal key) (Ghost.reveal iv) ))) =
+  let taint_func (x:b8) : GTot taint =
+    if StrongExcludedMiddle.strong_excluded_middle (x == plain_b) then Secret else
+    if StrongExcludedMiddle.strong_excluded_middle (x == mask_b) then Secret else
+    if StrongExcludedMiddle.strong_excluded_middle (x == cipher_b) then Secret else
+    Public in
+  let buffers = stack_b::plain_b::mask_b::cipher_b::[] in
+  let (mem:mem) = {addrs = addrs; ptrs = buffers; hs = h0} in
+  let addr_plain_b = addrs plain_b in
+  let addr_mask_b = addrs mask_b in
+  let addr_cipher_b = addrs cipher_b in
+  let addr_stack:nat64 = addrs stack_b + 0 in
+  let regs = fun r -> begin match r with
+    | Rsp -> addr_stack
+    | Rcx -> addr_plain_b
+    | Rdx -> addr_mask_b
+    | R8 -> addr_cipher_b
+    | R9 -> offset
+    | _ -> init_regs r end in
+  let xmms = init_xmms in
+  let va_s0 = {ok = true; regs = regs; xmms = xmms; flags = 0; mem = mem; trace = []; memTaint = create_valid_memtaint mem buffers taint_func} in  
   length_t_eq (TBase TUInt64) stack_b;
   length_t_eq (TBase TUInt128) plain_b;
   length_t_eq (TBase TUInt128) mask_b;
@@ -81,11 +92,11 @@ B.length stack_b == 40 /\ live h0 stack_b /\ bufs_disjoint [stack_b;plain_b;mask
     (buffer_to_seq_quad32 cipher_b va_s0.mem.hs));
   let mask128 = BV.mk_buffer_view mask_b Views.view128 in
   assert (Seq.equal (buffer_as_seq (va_get_mem va_s0) mask_b) (BV.as_seq va_s0.mem.hs mask128));
-  BV.as_seq_sel h0 mask128 0;
+  BV.as_seq_sel h0 mask128 0;  
   ()
 
-let implies_post (va_s0:va_state) (va_sM:va_state) (va_fM:va_fuel) (plain_b:b8) (mask_b:b8) (cipher_b:b8) (offset:nat64) (num_blocks:Ghost.erased (nat64)) (key:Ghost.erased (aes_key_LE AES_128)) (iv:Ghost.erased (quad32))  (stack_b:b8) : Lemma
-  (requires pre_cond va_s0.mem.hs plain_b mask_b cipher_b offset num_blocks key iv /\ B.length stack_b == 40 /\ live va_s0.mem.hs stack_b /\ bufs_disjoint [stack_b;plain_b;mask_b;cipher_b]/\
+let implies_post (va_s0:va_state) (va_sM:va_state) (va_fM:va_fuel) (plain_b:s8) (mask_b:s8) (cipher_b:s8) (offset:nat64) (num_blocks:Ghost.erased (nat64)) (key:Ghost.erased (aes_key_LE AES_128)) (iv:Ghost.erased (quad32))  (stack_b:b8) : Lemma
+  (requires pre_cond va_s0.mem.hs plain_b mask_b cipher_b offset num_blocks key iv /\ B.length stack_b == 40 /\ live va_s0.mem.hs stack_b /\ buf_disjoint_from stack_b [plain_b;mask_b;cipher_b]/\
     va_post (va_code_gcm_load_xor_store_buffer_win ()) va_s0 va_sM va_fM stack_b plain_b mask_b cipher_b offset (Ghost.reveal num_blocks) (Ghost.reveal key) (Ghost.reveal iv) )
   (ensures post_cond va_s0.mem.hs va_sM.mem.hs plain_b mask_b cipher_b offset num_blocks key iv ) =
   length_t_eq (TBase TUInt64) stack_b;
@@ -106,9 +117,14 @@ let implies_post (va_s0:va_state) (va_sM:va_state) (va_fM:va_fuel) (plain_b:b8) 
   BV.as_seq_sel va_s0.mem.hs mask128 0;      
   ()
 
-val ghost_gcm_load_xor_store_buffer_win: plain_b:b8 -> mask_b:b8 -> cipher_b:b8 -> offset:nat64 -> num_blocks:Ghost.erased (nat64) -> key:Ghost.erased (aes_key_LE AES_128) -> iv:Ghost.erased (quad32) ->  stack_b:b8 -> (h0:HS.mem{pre_cond h0 plain_b mask_b cipher_b offset num_blocks key iv /\ B.length stack_b == 40 /\ live h0 stack_b /\ bufs_disjoint [stack_b;plain_b;mask_b;cipher_b]}) -> GTot (h1:HS.mem{post_cond h0 h1 plain_b mask_b cipher_b offset num_blocks key iv })
+val ghost_gcm_load_xor_store_buffer_win: plain_b:s8 -> mask_b:s8 -> cipher_b:s8 -> offset:nat64 -> num_blocks:Ghost.erased (nat64) -> key:Ghost.erased (aes_key_LE AES_128) -> iv:Ghost.erased (quad32) ->  stack_b:b8 -> (h0:HS.mem{pre_cond h0 plain_b mask_b cipher_b offset num_blocks key iv /\ B.length stack_b == 40 /\ live h0 stack_b /\ buf_disjoint_from stack_b [plain_b;mask_b;cipher_b]}) -> GTot (h1:HS.mem{post_cond h0 h1 plain_b mask_b cipher_b offset num_blocks key iv })
 
 let ghost_gcm_load_xor_store_buffer_win plain_b mask_b cipher_b offset num_blocks key iv stack_b h0 =
+  let taint_func (x:b8) : GTot taint =
+    if StrongExcludedMiddle.strong_excluded_middle (x == plain_b) then Secret else
+    if StrongExcludedMiddle.strong_excluded_middle (x == mask_b) then Secret else
+    if StrongExcludedMiddle.strong_excluded_middle (x == cipher_b) then Secret else
+    Public in
   let buffers = stack_b::plain_b::mask_b::cipher_b::[] in
   let (mem:mem) = {addrs = addrs; ptrs = buffers; hs = h0} in
   let addr_plain_b = addrs plain_b in
@@ -123,7 +139,7 @@ let ghost_gcm_load_xor_store_buffer_win plain_b mask_b cipher_b offset num_block
     | R9 -> offset
     | _ -> init_regs r end in
   let xmms = init_xmms in
-  let s0 = {ok = true; regs = regs; xmms = xmms; flags = 0; mem = mem} in
+  let s0 = {ok = true; regs = regs; xmms = xmms; flags = 0; mem = mem; trace = []; memTaint = create_valid_memtaint mem buffers taint_func} in
   length_t_eq (TBase TUInt64) stack_b;
   length_t_eq (TBase TUInt128) plain_b;
   length_t_eq (TBase TUInt128) mask_b;
@@ -161,5 +177,5 @@ let gcm_load_xor_store_buffer_win plain_b mask_b cipher_b offset num_blocks key 
   push_frame();
   let (stack_b:b8) = B.alloca (UInt8.uint_to_t 0) (UInt32.uint_to_t 40) in
   let h0 = get() in
-  st_put h0 (fun h -> pre_cond h plain_b mask_b cipher_b (UInt64.v offset) num_blocks key iv /\ B.length stack_b == 40 /\ live h stack_b /\ bufs_disjoint [stack_b;plain_b;mask_b;cipher_b]) (ghost_gcm_load_xor_store_buffer_win plain_b mask_b cipher_b (UInt64.v offset) num_blocks key iv stack_b);
+  st_put h0 (fun h -> pre_cond h plain_b mask_b cipher_b (UInt64.v offset) num_blocks key iv /\ B.length stack_b == 40 /\ live h stack_b /\ buf_disjoint_from stack_b [plain_b;mask_b;cipher_b]) (ghost_gcm_load_xor_store_buffer_win plain_b mask_b cipher_b (UInt64.v offset) num_blocks key iv stack_b);
   pop_frame()
