src/arch/x64/interop/Gcm_load_xor_win.fsti
@@ -8,6 +8,7 @@ module M = LowStar.Modifies
 open LowStar.ModifiesPat
 open FStar.HyperStack.ST
 module HS = FStar.HyperStack
+module S8 = SecretByte
 open Interop
 open Words_s
 open Types_s
@@ -19,8 +20,9 @@ open AES_s
 open GCTR_s
 open GCTR_i
 
+let s8 = B.buffer S8.t
 
-let buffer_to_quad32 (b:B.buffer UInt8.t { B.length b % 16 == 0 /\ B.length b > 0 }) (h:HS.mem) : GTot quad32 =
+let buffer_to_quad32 (b:s8 { B.length b % 16 == 0 /\ B.length b > 0 }) (h:HS.mem) : GTot quad32 =
   let b128 = BV.mk_buffer_view b Views.view128 in
   BV.as_buffer_mk_buffer_view b Views.view128;
   BV.get_view_mk_buffer_view b Views.view128;
@@ -30,7 +32,7 @@ let buffer_to_quad32 (b:B.buffer UInt8.t { B.length b % 16 == 0 /\ B.length b > 
   BV.sel h b128 0
   //index (BV.as_seq h b128) 0
 
-let buffer_to_seq_quad32 (b:B.buffer UInt8.t { B.length b % 16 == 0 }) (h:HS.mem) : GTot (s:Seq.seq quad32 {Seq.length s == B.length b / 16} ) =
+let buffer_to_seq_quad32 (b:s8{ B.length b % 16 == 0 }) (h:HS.mem) : GTot (s:Seq.seq quad32 {Seq.length s == B.length b / 16} ) =
   let b128 = BV.mk_buffer_view b Views.view128 in
   BV.as_buffer_mk_buffer_view b Views.view128;
   BV.get_view_mk_buffer_view b Views.view128;
@@ -38,24 +40,26 @@ let buffer_to_seq_quad32 (b:B.buffer UInt8.t { B.length b % 16 == 0 }) (h:HS.mem
   (BV.as_seq h b128)
 
 
-let rec loc_locs_disjoint_rec (l:b8) (ls:list b8) : Type0 =
+let rec loc_locs_disjoint_rec (l:s8) (ls:list s8) : Type0 =
   match ls with
   | [] -> True
   | h::t -> M.loc_disjoint (M.loc_buffer l) (M.loc_buffer h) /\ loc_locs_disjoint_rec l t
 
-let rec locs_disjoint_rec (ls:list b8) : Type0 =
+let rec locs_disjoint_rec (ls:list s8) : Type0 =
   match ls with
   | [] -> True
   | h::t -> loc_locs_disjoint_rec h t /\ locs_disjoint_rec t
 
 unfold
-let bufs_disjoint (ls:list b8) : Type0 = normalize (locs_disjoint_rec ls)
+let bufs_disjoint (ls:list s8) : Type0 = normalize (locs_disjoint_rec ls)
 
+unfold
+let buf_disjoint_from (b:s8) (ls:list s8) : Type0 = normalize (loc_locs_disjoint_rec b ls)
 
 open FStar.Mul
 
 // TODO: Complete with your pre- and post-conditions
-let pre_cond (h:HS.mem) (plain_b:b8) (mask_b:b8) (cipher_b:b8) (offset:nat64) (num_blocks:Ghost.erased (nat64)) (key:Ghost.erased (aes_key_LE AES_128)) (iv:Ghost.erased (quad32)) = live h plain_b /\ live h mask_b /\ live h cipher_b /\ bufs_disjoint [plain_b;mask_b;cipher_b] /\ length plain_b % 16 == 0 /\ length mask_b % 16 == 0 /\ length cipher_b % 16 == 0
+let pre_cond (h:HS.mem) (plain_b:s8) (mask_b:s8) (cipher_b:s8) (offset:nat64) (num_blocks:Ghost.erased (nat64)) (key:Ghost.erased (aes_key_LE AES_128)) (iv:Ghost.erased (quad32)) = live h plain_b /\ live h mask_b /\ live h cipher_b /\ bufs_disjoint [plain_b;mask_b;cipher_b] /\ length plain_b % 16 == 0 /\ length mask_b % 16 == 0 /\ length cipher_b % 16 == 0
  /\  ( let mods = M.loc_buffer cipher_b in  
     B.live h plain_b /\ B.live h mask_b /\ B.live h cipher_b /\
     M.loc_disjoint (M.loc_buffer plain_b) mods /\
@@ -78,7 +82,7 @@ let pre_cond (h:HS.mem) (plain_b:b8) (mask_b:b8) (cipher_b:b8) (offset:nat64) (n
     )
   )
 
-let post_cond (h:HS.mem) (h':HS.mem) (plain_b:b8) (mask_b:b8) (cipher_b:b8) (offset:nat64) (num_blocks:Ghost.erased (nat64)) (key:Ghost.erased (aes_key_LE AES_128)) (iv:Ghost.erased (quad32)) = length plain_b % 16 == 0 /\ length mask_b % 16 == 0 /\ length cipher_b % 16 == 0 /\
+let post_cond (h:HS.mem) (h':HS.mem) (plain_b:s8) (mask_b:s8) (cipher_b:s8) (offset:nat64) (num_blocks:Ghost.erased (nat64)) (key:Ghost.erased (aes_key_LE AES_128)) (iv:Ghost.erased (quad32)) = length plain_b % 16 == 0 /\ length mask_b % 16 == 0 /\ length cipher_b % 16 == 0 /\
     B.length plain_b  >= (Ghost.reveal num_blocks) * 16 /\
     B.length cipher_b == B.length plain_b /\
     B.length mask_b == 16 /\
@@ -98,6 +102,6 @@ let post_cond (h:HS.mem) (h':HS.mem) (plain_b:b8) (mask_b:b8) (cipher_b:b8) (off
     )
     )
 
-val gcm_load_xor_store_buffer_win: plain_b:b8 -> mask_b:b8 -> cipher_b:b8 -> offset:UInt64.t -> num_blocks:Ghost.erased (nat64) -> key:Ghost.erased (aes_key_LE AES_128) -> iv:Ghost.erased (quad32) -> Stack unit
+val gcm_load_xor_store_buffer_win: plain_b:s8 -> mask_b:s8 -> cipher_b:s8 -> offset:UInt64.t -> num_blocks:Ghost.erased (nat64) -> key:Ghost.erased (aes_key_LE AES_128) -> iv:Ghost.erased (quad32) -> Stack unit
 	(requires (fun h -> pre_cond h plain_b mask_b cipher_b (UInt64.v offset) num_blocks key iv ))
 	(ensures (fun h0 _ h1 -> post_cond h0 h1 plain_b mask_b cipher_b (UInt64.v offset) num_blocks key iv ))
