src/arch/x64/interop/Gcm_make_length_win.fsti
@@ -8,6 +8,7 @@ module M = LowStar.Modifies
 open LowStar.ModifiesPat
 open FStar.HyperStack.ST
 module HS = FStar.HyperStack
+module S8 = SecretByte
 open Interop
 open Words_s
 open Types_s
@@ -16,24 +17,28 @@ open X64.Memory_i_s
 open X64.Vale.State_i
 open X64.Vale.Decls_i
 
+let s8 = B.buffer S8.t
 
-let rec loc_locs_disjoint_rec (l:b8) (ls:list b8) : Type0 =
+let rec loc_locs_disjoint_rec (l:s8) (ls:list s8) : Type0 =
   match ls with
   | [] -> True
   | h::t -> M.loc_disjoint (M.loc_buffer l) (M.loc_buffer h) /\ loc_locs_disjoint_rec l t
 
-let rec locs_disjoint_rec (ls:list b8) : Type0 =
+let rec locs_disjoint_rec (ls:list s8) : Type0 =
   match ls with
   | [] -> True
   | h::t -> loc_locs_disjoint_rec h t /\ locs_disjoint_rec t
 
 unfold
-let bufs_disjoint (ls:list b8) : Type0 = normalize (locs_disjoint_rec ls)
+let bufs_disjoint (ls:list s8) : Type0 = normalize (locs_disjoint_rec ls)
+
+unfold
+let buf_disjoint_from (b:s8) (ls:list s8) : Type0 = normalize (loc_locs_disjoint_rec b ls)
 
 open FStar.Mul
 
 
-let buffer_to_quad32 (b:B.buffer UInt8.t { B.length b % 16 == 0 /\ B.length b > 0 }) (h:HS.mem) : GTot quad32 =
+let buffer_to_quad32 (b:s8 { B.length b % 16 == 0 /\ B.length b > 0 }) (h:HS.mem) : GTot quad32 =
   let b128 = BV.mk_buffer_view b Views.view128 in
   BV.as_buffer_mk_buffer_view b Views.view128;
   BV.get_view_mk_buffer_view b Views.view128;
@@ -43,19 +48,19 @@ let buffer_to_quad32 (b:B.buffer UInt8.t { B.length b % 16 == 0 /\ B.length b > 
   BV.sel h b128 0
 
 // TODO: Complete with your pre- and post-conditions
-let pre_cond (h:HS.mem) (plain_num_bytes:nat64) (auth_num_bytes:nat64) (b:b8) = 
+let pre_cond (h:HS.mem) (plain_num_bytes:nat64) (auth_num_bytes:nat64) (b:s8) = 
     B.live h b /\
     B.length b == 16 /\
     8 * plain_num_bytes < pow2_32 /\
     8 * auth_num_bytes < pow2_32
 
-let post_cond (h:HS.mem) (h':HS.mem) (plain_num_bytes:nat64) (auth_num_bytes:nat64) (b:b8) = 
+let post_cond (h:HS.mem) (h':HS.mem) (plain_num_bytes:nat64) (auth_num_bytes:nat64) (b:s8) = 
     8 * plain_num_bytes < pow2_32 /\
     8 * auth_num_bytes < pow2_32 /\
   length b == 16 /\     M.modifies (M.loc_buffer b) h h' /\
     (let new_b = buffer_to_quad32 b h' in
      new_b == reverse_bytes_quad32 (Mkfour (8 * plain_num_bytes) 0 (8 * auth_num_bytes) 0))
 
-val gcm_make_length_quad_buffer_win: plain_num_bytes:UInt64.t -> auth_num_bytes:UInt64.t -> b:b8 -> Stack unit
+val gcm_make_length_quad_buffer_win: plain_num_bytes:UInt64.t -> auth_num_bytes:UInt64.t -> b:s8 -> Stack unit
 	(requires (fun h -> pre_cond h (UInt64.v plain_num_bytes) (UInt64.v auth_num_bytes) b ))
 	(ensures (fun h0 _ h1 -> post_cond h0 h1 (UInt64.v plain_num_bytes) (UInt64.v auth_num_bytes) b ))
