src/arch/x64/interop/Inc32_win.fsti
@@ -8,6 +8,7 @@ module M = LowStar.Modifies
 open LowStar.ModifiesPat
 open FStar.HyperStack.ST
 module HS = FStar.HyperStack
+module S8 = SecretByte
 open Interop
 open Words_s
 open Types_s
@@ -17,23 +18,25 @@ open X64.Vale.State_i
 open X64.Vale.Decls_i
 open GCTR_s
 
-let rec loc_locs_disjoint_rec (l:b8) (ls:list b8) : Type0 =
+let s8 = B.buffer S8.t
+
+let rec loc_locs_disjoint_rec (l:s8) (ls:list s8) : Type0 =
   match ls with
   | [] -> True
   | h::t -> M.loc_disjoint (M.loc_buffer l) (M.loc_buffer h) /\ loc_locs_disjoint_rec l t
 
-let rec locs_disjoint_rec (ls:list b8) : Type0 =
+let rec locs_disjoint_rec (ls:list s8) : Type0 =
   match ls with
   | [] -> True
   | h::t -> loc_locs_disjoint_rec h t /\ locs_disjoint_rec t
 
 unfold
-let bufs_disjoint (ls:list b8) : Type0 = normalize (locs_disjoint_rec ls)
+let bufs_disjoint (ls:list s8) : Type0 = normalize (locs_disjoint_rec ls)
 
 unfold
-let buf_disjoint_from (b:b8) (ls:list b8) : Type0 = normalize (loc_locs_disjoint_rec b ls)
+let buf_disjoint_from (b:s8) (ls:list s8) : Type0 = normalize (loc_locs_disjoint_rec b ls)
 
-let buffer_to_quad32 (b:B.buffer UInt8.t { B.length b % 16 == 0 /\ B.length b > 0 }) (h:HS.mem) : GTot quad32 =
+let buffer_to_quad32 (b:s8 { B.length b % 16 == 0 /\ B.length b > 0 }) (h:HS.mem) : GTot quad32 =
   let b128 = BV.mk_buffer_view b Views.view128 in
   BV.as_buffer_mk_buffer_view b Views.view128;
   BV.get_view_mk_buffer_view b Views.view128;
@@ -43,17 +46,17 @@ let buffer_to_quad32 (b:B.buffer UInt8.t { B.length b % 16 == 0 /\ B.length b > 
   BV.sel h b128 0
 
 // TODO: Complete with your pre- and post-conditions
-let pre_cond (h:HS.mem) (iv_b:b8) =     
+let pre_cond (h:HS.mem) (iv_b:s8) =     
     B.live h iv_b /\
     B.length iv_b == 16
 
-let post_cond (h:HS.mem) (h':HS.mem) (iv_b:b8) =
+let post_cond (h:HS.mem) (h':HS.mem) (iv_b:s8) =
     B.length iv_b == 16 /\
     M.modifies (M.loc_buffer iv_b) h h' /\
     (let old_iv = buffer_to_quad32 iv_b h  in
      let new_iv = buffer_to_quad32 iv_b h' in
      new_iv == inc32 old_iv 1)
 
-val inc32_buffer_win: iv_b:b8 -> Stack unit
+val inc32_buffer_win: iv_b:s8 -> Stack unit
 	(requires (fun h -> pre_cond h iv_b ))
 	(ensures (fun h0 _ h1 -> post_cond h0 h1 iv_b ))
