src/arch/x64/interop/Mk_quad32_1_win.fsti
@@ -8,6 +8,7 @@ module M = LowStar.Modifies
 open LowStar.ModifiesPat
 open FStar.HyperStack.ST
 module HS = FStar.HyperStack
+module S8 = SecretByte
 open Interop
 open Words_s
 open Types_s
@@ -17,8 +18,9 @@ open X64.Vale.State_i
 open X64.Vale.Decls_i
 #set-options "--z3rlimit 40"
 
+let s8 = B.buffer S8.t
 
-let buffer_to_quad32 (b:B.buffer UInt8.t { B.length b % 16 == 0 /\ B.length b > 0 }) (h:HS.mem) : GTot quad32 =
+let buffer_to_quad32 (b:s8 { B.length b % 16 == 0 /\ B.length b > 0 }) (h:HS.mem) : GTot quad32 =
   let b128 = BV.mk_buffer_view b Views.view128 in
   BV.as_buffer_mk_buffer_view b Views.view128;
   BV.get_view_mk_buffer_view b Views.view128;
@@ -28,17 +30,17 @@ let buffer_to_quad32 (b:B.buffer UInt8.t { B.length b % 16 == 0 /\ B.length b > 
   BV.sel h b128 0
 
 // TODO: Complete with your pre- and post-conditions
-let pre_cond (h:HS.mem) (b:b8) = 
+let pre_cond (h:HS.mem) (b:s8) = 
     B.live h b /\
     B.length b == 16
     
-let post_cond (h:HS.mem) (h':HS.mem) (b:b8) =
+let post_cond (h:HS.mem) (h':HS.mem) (b:s8) =
     B.length b == 16 /\
       M.modifies (M.loc_buffer b) h h' /\
     (let old_b = buffer_to_quad32 b h  in
      let new_b = buffer_to_quad32 b h' in
      new_b == Mkfour 1 old_b.lo1 old_b.hi2 old_b.hi3)
 
-val mk_quad32_lo0_be_1_buffer_win: b:b8 -> Stack unit
+val mk_quad32_lo0_be_1_buffer_win: b:s8 -> Stack unit
 	(requires (fun h -> pre_cond h b ))
 	(ensures (fun h0 _ h1 -> post_cond h0 h1 b ))
