src/arch/x64/interop/Vale_aes128_encrypt_block_be_win.fst
@@ -24,7 +24,7 @@ let va_code_aes128_encrypt_block_be_win () = va_code_AESEncryptBlockStdcall_BE i
 let vale_pre (va_b0:va_code) (va_s0:va_state) (win:bool) (alg:algorithm)
   (input:quad32) (key:(aes_key_LE alg)) (input_buffer:buffer128) (output_buffer:buffer128)
   (keys_buffer:buffer128) =
-  ((va_require_total va_b0 (va_code_AESEncryptBlockStdcall_BE win alg) va_s0) /\
+((va_require_total va_b0 (va_code_AESEncryptBlockStdcall_BE win alg) va_s0) /\
     (va_get_ok va_s0) /\ (let output_ptr = (if win then (va_get_reg Rcx va_s0) else (va_get_reg Rdi
     va_s0)) in let input_ptr = (if win then (va_get_reg Rdx va_s0) else (va_get_reg Rsi va_s0)) in
     let expanded_key_ptr = (if win then (va_get_reg R8 va_s0) else (va_get_reg Rdx va_s0)) in
@@ -33,8 +33,9 @@ let vale_pre (va_b0:va_code) (va_s0:va_state) (win:bool) (alg:algorithm)
     output_buffer input_buffer) (output_buffer == input_buffer)) /\ (alg = AES_128 || alg =
     AES_256) /\ (buffer128_read input_buffer 0 (va_get_mem va_s0)) == input /\ expanded_key_ptr ==
     (buffer_addr keys_buffer (va_get_mem va_s0)) /\ (validSrcAddrs128 (va_get_mem va_s0) input_ptr
-    input_buffer 1) /\ (validSrcAddrs128 (va_get_mem va_s0) output_ptr output_buffer 1) /\
-    (validSrcAddrs128 (va_get_mem va_s0) expanded_key_ptr keys_buffer ((nr alg) + 1)) /\ (forall
+    input_buffer 1 (va_get_memTaint va_s0) Secret) /\ (validSrcAddrs128 (va_get_mem va_s0)
+    output_ptr output_buffer 1 (va_get_memTaint va_s0) Secret) /\ (validSrcAddrs128 (va_get_mem
+    va_s0) expanded_key_ptr keys_buffer ((nr alg) + 1) (va_get_memTaint va_s0) Secret) /\ (forall
     (i:int) . (0 <= i && i < (nr alg) + 1) ==> (buffer128_read keys_buffer i (va_get_mem va_s0)) ==
     (index (key_to_round_keys_LE alg key) i))))
 
@@ -52,11 +53,12 @@ let vale_post (va_b0:va_code) (va_s0:va_state) (win:bool) (alg:algorithm)
     input_ptr = (if win then (va_get_reg Rdx va_s0) else (va_get_reg Rsi va_s0)) in let
     expanded_key_ptr = (if win then (va_get_reg R8 va_s0) else (va_get_reg Rdx va_s0)) in
     (modifies_mem (loc_buffer output_buffer) (va_get_mem va_s0) (va_get_mem va_sM)) /\
-    (validSrcAddrs128 (va_get_mem va_sM) output_ptr output_buffer 1) /\ (buffer128_read
-    output_buffer 0 (va_get_mem va_sM)) == (aes_encrypt_BE alg key input)) /\ (va_state_eq va_sM
-    (va_update_flags va_sM (va_update_xmm 2 va_sM (va_update_xmm 0 va_sM (va_update_mem va_sM
-    (va_update_reg Rax va_sM (va_update_reg R8 va_sM (va_update_ok va_sM va_s0)))))))))
-
+    (validSrcAddrs128 (va_get_mem va_sM) output_ptr output_buffer 1 (va_get_memTaint va_sM) Secret)
+    /\ (buffer128_read output_buffer 0 (va_get_mem va_sM)) == (aes_encrypt_BE alg key input)) /\
+    (va_state_eq va_sM (va_update_trace va_sM (va_update_flags va_sM (va_update_xmm 2 va_sM
+    (va_update_xmm 0 va_sM (va_update_mem va_sM (va_update_reg Rax va_sM (va_update_reg R8 va_sM
+    (va_update_ok va_sM va_s0))))))))))
+    
 let va_post (va_b0:va_code) (va_s0:va_state) (va_sM:va_state) (va_fM:va_fuel) (stack_b:buffer64)
   (output_b:buffer128) (input_b:buffer128) (key:(aes_key_LE AES_128)) (keys_b:buffer128) =
   vale_post va_b0 va_s0 is_win AES_128
